start on new ElimFuncComp2

src/ElimFunc2.v
@@ -1,12 +1,11 @@
 Require Import Common.
-Require Import StepLib.
 
 Require Import Utopia.
 Require Import Monads.
 Require Import ListLemmas.
-Require Import Psatz.
+Require Import Metadata.
 Require Import HigherValue.
-
+Require StepLib.
 
 Definition function_name := nat.
 
@@ -17,33 +16,106 @@ Definition rec_info := list bool.
 
 Inductive expr :=
 | Value (v : value)
-| Arg : expr
-| UpVar : nat -> expr
-| Call : expr -> expr -> expr
+| Arg
+| UpVar (idx : nat)
+| Call (f : expr) (a : expr)
 | MkConstr (tag : nat) (args : list expr)
-| ElimBody (rec : expr) (cases : list (expr * rec_info))
+| Elim (loop : expr) (cases : list (expr * rec_info)) (target : expr)
 | MkClose (f : function_name) (free : list expr)
 .
-
-Definition env := list expr.
 
 Inductive is_value : expr -> Prop :=
 | IsValue : forall v, is_value (Value v).
 
+Definition env := list expr.
 
-Fixpoint unroll_elim (rec : expr)
-                     (case : expr)
+Fixpoint unroll_elim (case : expr)
                      (args : list value)
-                     (info : rec_info) : option expr :=
-    match args, info with
+                     (rec : rec_info)
+                     (mk_rec : expr -> expr) : option expr :=
+    match args, rec with
     | [], [] => Some case
-    | arg :: args, r :: info =>
+    | arg :: args, r :: rec =>
             let case := Call case (Value arg) in
-            let case := if r then Call case (Call rec (Value arg)) else case in
-            unroll_elim rec case args info
+            let case := if r then Call case (mk_rec (Value arg)) else case in
+            unroll_elim case args rec mk_rec
     | _, _ => None
     end.
 
+
+Inductive state :=
+| Run (e : expr) (l : list value) (k : value -> state)
+| Stop (v : value).
+
+Inductive sstep (E : env) : state -> state -> Prop :=
+| SArg : forall l k v,
+        nth_error l 0 = Some v ->
+        sstep E (Run Arg l k) (k v)
+| SUpVar : forall n l k v,
+        nth_error l (S n) = Some v ->
+        sstep E (Run (UpVar n) l k) (k v)
+
+| SCloseStep : forall tag vs e es l k,
+        Forall is_value vs ->
+        ~ is_value e ->
+        sstep E (Run (MkClose tag (vs ++ [e] ++ es)) l k)
+                (Run e l (fun v => Run (MkClose tag (vs ++ [Value v] ++ es)) l k))
+| SCloseDone : forall tag vs l k,
+        let es := map Value vs in
+        sstep E (Run (MkClose tag es) l k) (k (Close tag vs))
+
+| SConstrStep : forall fname vs e es l k,
+        Forall is_value vs ->
+        ~ is_value e ->
+        sstep E (Run (MkConstr fname (vs ++ [e] ++ es)) l k)
+                (Run e l (fun v => Run (MkConstr fname (vs ++ [Value v] ++ es)) l k))
+| SConstrDone : forall fname vs l k,
+        let es := map Value vs in
+        sstep E (Run (MkConstr fname es) l k) (k (Constr fname vs))
+
+| SCallL : forall e1 e2 l k,
+        ~ is_value e1 ->
+        sstep E (Run (Call e1 e2) l k)
+                (Run e1 l (fun v => Run (Call (Value v) e2) l k))
+| SCallR : forall e1 e2 l k,
+        is_value e1 ->
+        ~ is_value e2 ->
+        sstep E (Run (Call e1 e2) l k)
+                (Run e2 l (fun v => Run (Call e1 (Value v)) l k))
+| SMakeCall : forall fname free arg l k body,
+        nth_error E fname = Some body ->
+        sstep E (Run (Call (Value (Close fname free)) (Value arg)) l k)
+                (Run body (arg :: free) k)
+
+| SElimStepLoop : forall loop cases target l k,
+        ~ is_value loop ->
+        sstep E (Run (Elim loop cases target) l k)
+                (Run loop l (fun v => Run (Elim (Value v) cases target) l k))
+| SElimStep : forall loop cases target l k,
+        is_value loop ->
+        ~ is_value target ->
+        sstep E (Run (Elim loop cases target) l k)
+                (Run target l (fun v => Run (Elim loop cases (Value v)) l k))
+| SEliminate : forall loop cases tag args l k case rec e',
+        is_value loop ->
+        nth_error cases tag = Some (case, rec) ->
+        unroll_elim case args rec (fun x => Call loop x) = Some e' ->
+        sstep E (Run (Elim loop cases (Value (Constr tag args))) l k)
+                (Run e' l k)
+.
+
+Definition sstar BE := StepLib.sstar (sstep BE).
+Definition SStarNil := @StepLib.SStarNil state.
+Definition SStarCons := @StepLib.SStarCons state.
+
+Definition splus BE := StepLib.splus (sstep BE).
+Definition SPlusOne := @StepLib.SPlusOne state.
+Definition SPlusCons := @StepLib.SPlusCons state.
+
+
+
+
+(* Proofs *)
 
 (*
  * Mutual recursion/induction schemes for expr
@@ -59,7 +131,8 @@ Definition expr_rect_mut
     (HUpVar :   forall n, P (UpVar n))
     (HCall :    forall f a, P f -> P a -> P (Call f a))
     (HConstr :  forall tag args, Pl args -> P (MkConstr tag args))
-    (HElimBody : forall rec cases, P rec -> Plp cases -> P (ElimBody rec cases))
+    (HElim :    forall loop cases target,
+        P loop -> Plp cases -> P target -> P (Elim loop cases target))
     (HClose :   forall f free, Pl free -> P (MkClose f free))
     (Hnil :     Pl [])
     (Hcons :    forall e es, P e -> Pl es -> Pl (e :: es))
@@ -87,7 +160,8 @@ Definition expr_rect_mut
         | UpVar n => HUpVar n
         | Call f a => HCall f a (go f) (go a)
         | MkConstr tag args => HConstr tag args (go_list args)
-        | ElimBody rec cases => HElimBody rec cases (go rec) (go_pair_list cases)
+        | Elim loop cases target =>
+                HElim loop cases target (go loop) (go_pair_list cases) (go target)
         | MkClose f free => HClose f free (go_list free)
         end in go e.
 
@@ -96,25 +170,11 @@ Definition expr_rect_mut'
         (Pl : list expr -> Type)
         (Pp : expr * rec_info -> Type)
         (Plp : list (expr * rec_info) -> Type)
-    (HValue :   forall v, P (Value v))
-    (HArg :     P Arg)
-    (HUpVar :   forall n, P (UpVar n))
-    (HCall :    forall f a, P f -> P a -> P (Call f a))
-    (HConstr :  forall tag args, Pl args -> P (MkConstr tag args))
-    (HElimBody : forall rec cases, P rec -> Plp cases -> P (ElimBody rec cases))
-    (HClose :   forall f free, Pl free -> P (MkClose f free))
-    (Hnil :     Pl [])
-    (Hcons :    forall e es, P e -> Pl es -> Pl (e :: es))
-    (Hpair :    forall e r, P e -> Pp (e, r))
-    (Hnil_p :   Plp [])
-    (Hcons_p :  forall p ps, Pp p -> Plp ps -> Plp (p :: ps)) :
-    (forall e, P e) *
-    (forall es, Pl es) *
-    (forall p, Pp p) *
-    (forall ps, Plp ps) :=
+    HValue HArg HUpVar HCall HConstr HElim HClose Hnil Hcons Hpair Hnil_p Hcons_p
+    : (forall e, P e) * (forall es, Pl es) * (forall p, Pp p) * (forall ps, Plp ps) :=
     let go := expr_rect_mut P Pl Pp Plp
-        HValue HArg HUpVar HCall HConstr HElimBody HClose
-        Hnil Hcons Hpair Hnil_p Hcons_p in
+        HValue HArg HUpVar HCall HConstr HElim HClose Hnil Hcons Hpair Hnil_p Hcons_p
+    in
     let fix go_list es :=
         match es as es_ return Pl es_ with
         | [] => Hnil
@@ -123,12 +183,12 @@ Definition expr_rect_mut'
     let go_pair p :=
         let '(e, r) := p in
         Hpair e r (go e) in
-    let fix go_list_pair ps :=
+    let fix go_pair_list ps :=
         match ps as ps_ return Plp ps_ with
         | [] => Hnil_p
-        | p :: ps => Hcons_p p ps (go_pair p) (go_list_pair ps)
+        | p :: ps => Hcons_p p ps (go_pair p) (go_pair_list ps)
         end in
-    (go, go_list, go_pair, go_list_pair).
+    (go, go_list, go_pair, go_pair_list).
 
 (* Useful wrapper for `expr_rect_mut with (Pl := Forall P)` *)
 Definition expr_ind' (P : expr -> Prop) (Pp : (expr * rec_info) -> Prop)
@@ -137,13 +197,13 @@ Definition expr_ind' (P : expr -> Prop) (Pp : (expr * rec_info) -> Prop)
     (HUpVar :   forall n, P (UpVar n))
     (HCall :    forall f a, P f -> P a -> P (Call f a))
     (HConstr :  forall c args, Forall P args -> P (MkConstr c args))
-    (HElimBody : forall rec cases,
-        P rec -> Forall Pp cases -> P (ElimBody rec cases))
+    (HElim :    forall loop cases target,
+        P loop -> Forall Pp cases -> P target -> P (Elim loop cases target))
     (HClose :   forall f free, Forall P free -> P (MkClose f free))
     (Hpair :    forall e r, P e -> Pp (e, r))
     (e : expr) : P e :=
     ltac:(refine (@expr_rect_mut P (Forall P) Pp (Forall Pp)
-        HValue HArg HUpVar HCall HConstr HElimBody HClose _ _ Hpair _ _ e); eauto).
+        HValue HArg HUpVar HCall HConstr HElim HClose _ _ Hpair _ _ e); eauto).
 
 (* Useful wrapper for `expr_rect_mut with (Pl := Forall P)` *)
 Definition expr_ind'' (P : expr -> Prop)
@@ -152,182 +212,51 @@ Definition expr_ind'' (P : expr -> Prop)
     (HUpVar :   forall n, P (UpVar n))
     (HCall :    forall f a, P f -> P a -> P (Call f a))
     (HConstr :  forall c args, Forall P args -> P (MkConstr c args))
-    (HElimBody : forall rec cases,
-        P rec ->
+    (HElim :    forall loop cases target,
+        P loop ->
         Forall (fun c => P (fst c)) cases ->
-        P (ElimBody rec cases))
+        P target ->
+        P (Elim loop cases target))
     (HClose :   forall f free, Forall P free -> P (MkClose f free))
     (e : expr) : P e :=
     ltac:(refine (@expr_rect_mut P (Forall P) (fun c => P (fst c)) (Forall (fun c => P (fst c)))
-        HValue HArg HUpVar HCall HConstr HElimBody HClose _ _ _ _ _ e); eauto).
+        HValue HArg HUpVar HCall HConstr HElim HClose _ _ _ _ _ e); eauto).
 
 
+(*
+ * Misc lemmas
+ *)
 
-Definition num_locals :=
-    let fix go e :=
-        let fix go_list es :=
-            match es with
-            | [] => 0
-            | e :: es => max (go e) (go_list es)
-            end in
-        let fix go_pair p :=
-            match p with
-            | (e, _) => go e
-            end in
-        let fix go_list_pair ps :=
-            match ps with
-            | [] => 0
-            | p :: ps => max (go_pair p) (go_list_pair ps)
-            end in
-        match e with
-        | Value v => 0
-        | Arg => 1
-        | UpVar i => S (S i)
-        | Call f a => max (go f) (go a)
-        | MkConstr _ args => go_list args
-        (* Recall: ElimBody implicitly accesses Arg, and removes it before running cases *)
-        | ElimBody rec cases => max (max (go rec) (S (go_list_pair cases))) 1
-        | MkClose _ free => go_list free
-        end in go.
+Lemma unroll_elim_length : forall case args rec mk_rec,
+    length args = length rec <-> unroll_elim case args rec mk_rec <> None.
+first_induction args; destruct rec; intros; split; simpl;
+  try solve [intro; congruence].
 
-(* Nested fixpoint aliases *)
-Definition num_locals_list :=
-    let go := num_locals in
-    let fix go_list es :=
-        match es with
-        | [] => 0
-        | e :: es => max (go e) (go_list es)
-        end in go_list.
-
-Definition num_locals_pair :=
-    let go := num_locals in
-    let fix go_pair (p : expr * rec_info) :=
-        match p with
-        | (e, _) => go e
-        end in go_pair.
-
-Definition num_locals_list_pair :=
-    let go_pair := num_locals_pair in
-    let fix go_list_pair ps :=
-        match ps with
-        | [] => 0
-        | p :: ps => max (go_pair p) (go_list_pair ps)
-        end in go_list_pair.
-
-Ltac refold_num_locals :=
-    fold num_locals_list in *;
-    fold num_locals_pair in *;
-    fold num_locals_list_pair in *.
-
-Lemma num_locals_list_is_maximum : forall es,
-    num_locals_list es = maximum (map num_locals es).
-induction es; simpl in *; eauto.
+- intro Hlen. simpl. eapply IHargs. congruence.
+- intro Hcall. f_equal. apply <- IHargs. eauto.
 Qed.
 
-Lemma num_locals_list_pair_is_maximum : forall es,
-    num_locals_list_pair es = maximum (map (fun p => num_locals (fst p)) es).
-induction es; simpl in *; try destruct a; eauto.
-Qed.
-
-Lemma value_num_locals : forall e, is_value e -> num_locals e = 0.
-inversion 1. reflexivity.
-Qed.
-
-Lemma unroll_elim_num_locals : forall rec case args info e',
-    unroll_elim rec case args info = Some e' ->
-    num_locals e' <= max (num_locals rec) (num_locals case).
-first_induction args; destruct info; intros0 Hunroll; try discriminate; simpl in *; inject_some.
-- lia.
-- destruct b; specialize (IHargs ?? ?? ?? ?? **); simpl in *; refold_num_locals.
-  + repeat rewrite Nat.max_le_iff in *. firstorder.
-  + repeat rewrite Nat.max_le_iff in *. firstorder.
+Lemma length_unroll_elim : forall case args rec mk_rec,
+    length args = length rec ->
+    exists e, unroll_elim case args rec mk_rec = Some e.
+first_induction args; destruct rec; intros0 Hlen; simpl in Hlen; try discriminate Hlen.
+- eexists. reflexivity.
+- inv Hlen.
+  fwd eapply IHargs; try eassumption.
 Qed.
 
 
-
-(* Continuation-based step relation *)
-
-Inductive state :=
-| Run (e : expr) (l : list value) (k : value -> state)
-| Stop (e : value).
-
-Inductive sstep (E : env) : state -> state -> Prop :=
-| SArg : forall l k v,
-        nth_error l 0 = Some v ->
-        sstep E (Run Arg l k) (k v)
-| SUpVar : forall n l k v,
-        nth_error l (S n) = Some v ->
-        sstep E (Run (UpVar n) l k) (k v)
-
-| SCloseStep : forall fname vs e es l k,
-        Forall is_value vs ->
-        ~ is_value e ->
-        sstep E (Run (MkClose fname (vs ++ [e] ++ es)) l k)
-                (Run e l (fun v => Run (MkClose fname (vs ++ [Value v] ++ es)) l k))
-| SCloseDone : forall fname vs l k,
-        let es := map Value vs in
-        sstep E (Run (MkClose fname es) l k) (k (Close fname vs))
-
-| SConstrStep : forall fname vs e es l k,
-        Forall is_value vs ->
-        ~ is_value e ->
-        sstep E (Run (MkConstr fname (vs ++ [e] ++ es)) l k)
-                (Run e l (fun v => Run (MkConstr fname (vs ++ [Value v] ++ es)) l k))
-| SConstrDone : forall fname vs l k,
-        let es := map Value vs in
-        sstep E (Run (MkConstr fname es) l k) (k (Constr fname vs))
-
-| SCallL : forall e1 e2 l k,
-        ~ is_value e1 ->
-        sstep E (Run (Call e1 e2) l k)
-                (Run e1 l (fun v => Run (Call (Value v) e2) l k))
-| SCallR : forall e1 e2 l k,
-        is_value e1 ->
-        ~ is_value e2 ->
-        sstep E (Run (Call e1 e2) l k)
-                (Run e2 l (fun v => Run (Call e1 (Value v)) l k))
-| SMakeCall : forall fname free arg l k body,
-        nth_error E fname = Some body ->
-        sstep E (Run (Call (Value (Close fname free)) (Value arg)) l k)
-                (Run body (arg :: free) k)
-
-| SElimStepRec : forall rec cases l k,
-        ~ is_value rec ->
-        sstep E (Run (ElimBody rec cases) l k)
-                (Run rec l (fun v => Run (ElimBody (Value v) cases) l k))
-| SEliminate : forall rec cases tag args l k case info e',
-        is_value rec ->
-        nth_error cases tag = Some (case, info) ->
-        unroll_elim rec case args info = Some e' ->
-        (* XXX this step *removes* the scrutinee from the local context!
-           This is super janky but it makes the incoming match_states much
-           easier, because it means the contexts match exactly after entering
-           the actual case. *)
-        sstep E (Run (ElimBody rec cases) (Constr tag args :: l) k)
-                (Run e' l k)
-.
-
-
-
-Definition sstar BE := StepLib.sstar (sstep BE).
-Definition SStarNil := @StepLib.SStarNil state.
-Definition SStarCons := @StepLib.SStarCons state.
-
-Definition splus BE := StepLib.splus (sstep BE).
-Definition SPlusOne := @StepLib.SPlusOne state.
-Definition SPlusCons := @StepLib.SPlusCons state.
-
-
-
-Require Import Metadata.
+Require Semantics.
 
 Definition prog_type : Type := list expr * list metadata.
 Definition valtype := HigherValue.value.
 
+Definition initial_env (prog : prog_type) : env := fst prog.
+
 Inductive is_callstate (prog : prog_type) : valtype -> valtype -> state -> Prop :=
 | IsCallstate : forall fname free av body,
         nth_error (fst prog) fname = Some body ->
-        let fv := HigherValue.Close fname free in
+        let fv := Close fname free in
         HigherValue.public_value (snd prog) fv ->
         HigherValue.public_value (snd prog) av ->
         is_callstate prog fv av
@@ -338,687 +267,10 @@ Inductive final_state (prog : prog_type) : state -> valtype -> Prop :=
         HigherValue.public_value (snd prog) v ->
         final_state prog (Stop v) v.
 
-Definition initial_env (prog : prog_type) : env := fst prog.
-
 Definition semantics (prog : prog_type) : Semantics.semantics :=
   @Semantics.Semantics_gen state env valtype
-                           (is_callstate prog)
-                           
+                 (is_callstate prog)
                  (sstep)
-                 (* (initial_state prog) *)
                  (final_state prog)
                  (initial_env prog).
-
-
-
-Definition enough_free E :=
-    let fix go e :=
-        let fix go_list es :=
-            match es with
-            | [] => True
-            | e :: es => go e /\ go_list es
-            end in
-        let fix go_pair p :=
-            let '(e, r) := p in
-            go e in
-        let fix go_list_pair ps :=
-            match ps with
-            | [] => True
-            | p :: ps => go_pair p /\ go_list_pair ps
-            end in
-        match e with
-        | Value _ => True
-        | Arg => True
-        | UpVar _ => True
-        | Call f a => go f /\ go a
-        | MkConstr _ args => go_list args
-        | ElimBody rec cases => go rec /\ go_list_pair cases
-        | MkClose fname free => go_list free /\
-            exists body,
-                nth_error E fname = Some body /\
-                num_locals body <= S (length free)
-        end in go.
-
-Definition enough_free_list E :=
-    let go := enough_free E in
-    let fix go_list es :=
-        match es with
-        | [] => True
-        | e :: es => go e /\ go_list es
-        end in go_list.
-
-Definition enough_free_pair E :=
-    let go := enough_free E in
-    let fix go_pair (p : expr * rec_info) :=
-        match p with
-        | (e, _) => go e
-        end in go_pair.
-
-Definition enough_free_list_pair E :=
-    let go_pair := enough_free_pair E in
-    let fix go_list_pair ps :=
-        match ps with
-        | [] => True
-        | p :: ps => go_pair p /\ go_list_pair ps
-        end in go_list_pair.
-
-Ltac refold_enough_free E :=
-    fold (enough_free_list E) in *;
-    fold (enough_free_pair E) in *;
-    fold (enough_free_list_pair E) in *.
-
-Inductive enough_free_state E : state -> Prop :=
-| EfsRun : forall e l k,
-        enough_free E e ->
-        (forall v, enough_free_state E (k v)) ->
-        enough_free_state E (Run e l k)
-| EfsStop : forall v,
-        enough_free_state E (Stop v).
-
-Lemma enough_free_list_Forall : forall E es,
-    enough_free_list E es <-> Forall (enough_free E) es.
-induction es; split; intro HH.
-- constructor.
-- constructor.
-- invc HH. constructor; firstorder.
-- invc HH. constructor; firstorder.
-Qed.
-
-Lemma enough_free_list_pair_Forall : forall E ps,
-    enough_free_list_pair E ps <-> Forall (fun p => enough_free E (fst p)) ps.
-induction ps; split; intro HH.
-- constructor.
-- constructor.
-- invc HH. destruct a. constructor; firstorder.
-- invc HH. destruct a. constructor; firstorder.
-Qed.
-
-
-
-Ltac efd_fixup E := simpl; refold_enough_free E;
-    try rewrite enough_free_list_Forall;
-    try rewrite enough_free_list_pair_Forall.
-
-Ltac efd_fail E := right; efd_fixup E; inversion 1; eauto.
-
-Definition enough_free_dec E e : { enough_free E e } + { ~ enough_free E e }.
-induction e using expr_rect_mut with
-    (Pl := fun es => { Forall (enough_free E) es } + { ~ Forall (enough_free E) es })
-    (Pp := fun p => { enough_free E (fst p) } + { ~ enough_free E (fst p) })
-    (Plp := fun ps => { Forall (fun p => enough_free E (fst p)) ps } +
-                      { ~ Forall (fun p => enough_free E (fst p)) ps }).
-
-- left. constructor.
-- left. constructor.
-- left. constructor.
-- destruct IHe1; [ | efd_fail E ].
-  destruct IHe2; [ | efd_fail E ].
-  left. firstorder.
-- destruct IHe; [ | efd_fail E ].
-  left. efd_fixup E. firstorder.
-- destruct IHe; [ | efd_fail E ].
-  destruct IHe0; [ | efd_fail E ].
-  left. efd_fixup E. firstorder.
-- destruct IHe; [ | efd_fail E ].
-  destruct (nth_error E f) as [ body | ] eqn:?; cycle 1.
-    { right. inversion 1. refold_enough_free E. firstorder congruence. }
-  destruct (le_dec (num_locals body) (S (length free))); cycle 1.
-    { right. inversion 1. refold_enough_free E. break_exists. break_and.
-      replace x with body in * by congruence. lia. }
-  left. efd_fixup E. firstorder.
-
-- left. constructor.
-- destruct IHe; [ | efd_fail E ].
-  destruct IHe0; [ | efd_fail E ].
-  left. efd_fixup E. firstorder.
-
-- simpl. assumption.
-
-- left. constructor.
-- destruct IHe; [ | efd_fail E ].
-  destruct IHe0; [ | efd_fail E ].
-  left. efd_fixup E. firstorder.
-Defined.
-
-Definition enough_free_list_dec E e : { enough_free_list E e } + { ~ enough_free_list E e }.
-induction e.
-- left. constructor.
-- destruct (enough_free_dec E a); [ | right; inversion 1; auto ].
-  destruct IHe; [ | right; inversion 1; auto ].
-  left. constructor; auto.
-Defined.
-
-
-
-Lemma enough_free_unroll_elim : forall E rec case args info e',
-    unroll_elim rec case args info = Some e' ->
-    enough_free E rec ->
-    enough_free E case ->
-    enough_free E e'.
-first_induction args; destruct info; intros0 Hunroll EFrec EFcase; try discriminate.
-  { simpl in *. congruence. }
-
-simpl in *. refold_enough_free E.
-destruct b.
-- eapply IHargs; try eassumption.
-  simpl. auto.
-- eapply IHargs; try eassumption.
-  simpl. auto.
-Qed.
-
-Lemma enough_free_step : forall E s s',
-    Forall (enough_free E) E ->
-    enough_free_state E s ->
-    sstep E s s' ->
-    enough_free_state E s'.
-intros0 Henv Hefs Hstep. invc Hstep; invc Hefs.
-
-- (* SArg *)
-  eapply H4.
-
-- (* SUpVar *)
-  eapply H4.
-
-- (* SCloseStep *)
-  on (enough_free _ _), invc. refold_enough_free E. rewrite enough_free_list_Forall in *.
-  on (Forall _ (_ ++ _ :: _)), invc_using Forall_3part_inv.
-
-  constructor; eauto.
-  intros. constructor; eauto.
-  simpl. refold_enough_free E. rewrite enough_free_list_Forall.
-  rewrite app_length in *. simpl in *.
-  split; [|assumption].
-  eapply Forall_app; eauto. eapply Forall_cons; eauto. constructor.
-
-- (* SCloseDone *) eauto.
-
-- (* SConstrStep *)
-  simpl in *. refold_enough_free E. rewrite enough_free_list_Forall in *.
-  on (Forall _ (_ ++ _ :: _)), invc_using Forall_3part_inv.
-
-  constructor; eauto.
-  intros. constructor; eauto.
-  simpl. refold_enough_free E. rewrite enough_free_list_Forall.
-  eapply Forall_app; eauto. eapply Forall_cons; eauto. constructor.
-
-- (* SConstrDone *) eauto.
-
-- (* SCallL *)
-  on (enough_free _ _), invc.
-  constructor; eauto.
-  intros. constructor; eauto.
-  split; [constructor | assumption].
-
-- (* SCallR *)
-  on (enough_free _ _), invc.
-  constructor; eauto.
-  intros. constructor; eauto.
-  split; [assumption | constructor].
-
-- (* SMakeCall *)
-  constructor; eauto.
-    { eapply Forall_nth_error with (xs := E); eassumption. }
-
-- (* SElimStepRec *)
-  on (enough_free _ _), invc. refold_enough_free E.
-  constructor; eauto.
-  intros. constructor; eauto.
-  simpl. refold_enough_free E. eauto.
-
-- (* SEliminate *)
-  on (enough_free _ _), invc. refold_enough_free E.
-
-  fwd eapply enough_free_unroll_elim; try eassumption; eauto.
-    { cut (enough_free_pair E (case, info)); [ simpl; intro; assumption | ].
-      rewrite enough_free_list_pair_Forall in *.
-      eapply Forall_nth_error; [ | eassumption ].
-      list_magic_on (cases, tt). destruct cases_i. auto. }
-
-  constructor; eauto.
-Qed.
-
-Lemma enough_free_plus : forall E s s',
-    Forall (enough_free E) E ->
-    enough_free_state E s ->
-    splus E s s' ->
-    enough_free_state E s'.
-induction 3; eauto using enough_free_step.
-Qed.
-
-Lemma enough_free_star : forall E s s',
-    Forall (enough_free E) E ->
-    enough_free_state E s ->
-    sstar E s s' ->
-    enough_free_state E s'.
-induction 3; eauto using enough_free_step.
-Qed.
-
-
-Definition no_elim_body :=
-    let fix go e :=
-        let fix go_list es :=
-            match es with
-            | [] => True
-            | e :: es => go e /\ go_list es
-            end in
-        match e with
-        | Value v => True
-        | Arg => True
-        | UpVar _ => True
-        | Call f a => go f /\ go a
-        | MkConstr _ args => go_list args
-        | ElimBody _ _ => False
-        | MkClose _ free => go_list free
-        end in go.
-
-Definition no_elim_body_list :=
-    let go := no_elim_body in
-    let fix go_list es :=
-        match es with
-        | [] => True
-        | e :: es => go e /\ go_list es
-        end in go_list.
-
-Definition no_elim_body_pair :=
-    let go := no_elim_body in
-    let fix go_pair (p : expr * rec_info) :=
-        match p with
-        | (e, _) => go e
-        end in go_pair.
-
-Definition no_elim_body_list_pair :=
-    let go_pair := no_elim_body_pair in
-    let fix go_list_pair ps :=
-        match ps with
-        | [] => True
-        | p :: ps => go_pair p /\ go_list_pair ps
-        end in go_list_pair.
-
-Ltac refold_no_elim_body :=
-    fold no_elim_body_list in *;
-    fold no_elim_body_pair in *;
-    fold no_elim_body_list_pair in *.
-
-Definition elim_body_placement e :=
-    match e with
-    | ElimBody rec cases => no_elim_body rec /\ no_elim_body_list_pair cases
-    | _ => no_elim_body e
-    end.
-
-Lemma no_elim_body_list_Forall : forall es,
-    no_elim_body_list es <-> Forall no_elim_body es.
-induction es; split; intro HH.
-- constructor.
-- constructor.
-- invc HH. constructor; firstorder.
-- invc HH. constructor; firstorder.
-Qed.
-
-Lemma no_elim_body_list_pair_Forall : forall ps,
-    no_elim_body_list_pair ps <-> Forall (fun p => no_elim_body (fst p)) ps.
-induction ps; split; intro HH.
-- constructor.
-- constructor.
-- invc HH. destruct a. constructor; firstorder.
-- invc HH. destruct a. constructor; firstorder.
-Qed.
-
-
-Ltac nebd_fail := right; (inversion 1 + simpl); eauto.
-
-Definition no_elim_body_dec e : { no_elim_body e } + { ~ no_elim_body e }.
-induction e using expr_rect_mut with
-    (Pl := fun es => { no_elim_body_list es } + { ~ no_elim_body_list es })
-    (Pp := fun p => { no_elim_body_pair p } + { ~ no_elim_body_pair p })
-    (Plp := fun ps => { no_elim_body_list_pair ps } + { ~ no_elim_body_list_pair ps });
-try solve [left; constructor | right; inversion 1].
-
-- destruct IHe1; [| nebd_fail ].
-  destruct IHe2; [| nebd_fail ].
-  left. constructor; auto.
-
-- destruct IHe; [| nebd_fail ].
-  left. auto.
-
-- destruct IHe; [| nebd_fail ].
-  left. auto.
-
-- destruct IHe; [| nebd_fail ].
-  destruct IHe0; [| nebd_fail ].
-  left. constructor; auto.
-
-- simpl. assumption.
-
-- destruct IHe; [| nebd_fail ].
-  destruct IHe0; [| nebd_fail ].
-  left. constructor; auto.
-Defined.
-
-Definition no_elim_body_list_dec es : { no_elim_body_list es } + { ~ no_elim_body_list es }.
-induction es.
-- left. constructor.
-- destruct (no_elim_body_dec a); [| nebd_fail ].
-  destruct IHes; [| nebd_fail ].
-  left. constructor; auto.
-Defined.
-
-Definition no_elim_body_pair_dec p : { no_elim_body_pair p } + { ~ no_elim_body_pair p }.
-destruct p.
-destruct (no_elim_body_dec e); [| nebd_fail ].
-left. auto.
-Defined.
-
-Definition no_elim_body_list_pair_dec ps :
-    { no_elim_body_list_pair ps } + { ~ no_elim_body_list_pair ps }.
-induction ps.
-- left. constructor.
-- destruct (no_elim_body_pair_dec a); [| nebd_fail ].
-  destruct IHps; [| nebd_fail ].
-  left. constructor; auto.
-Defined.
-
-
-Definition elim_body_placement_dec e : { elim_body_placement e } + { ~ elim_body_placement e }.
-destruct e; try eapply no_elim_body_dec.
-
-simpl.
-destruct (no_elim_body_dec e); [| nebd_fail ].
-destruct (no_elim_body_list_pair_dec cases); [| nebd_fail ].
-left. auto.
-Defined.
-
-Definition elim_body_placement_list_dec es :
-    { Forall elim_body_placement es } + { ~ Forall elim_body_placement es }.
-induction es.
-- left. constructor.
-- destruct (elim_body_placement_dec a); [| nebd_fail ].
-  destruct IHes; [| nebd_fail ].
-  left. constructor; auto.
-Defined.
-
-
-
-Definition shift :=
-    let fix go e :=
-        let fix go_list es :=
-            match es with
-            | [] => []
-            | e :: es => go e :: go_list es
-            end in
-        let fix go_pair p :=
-            let '(e, r) := p in
-            (go e, r) in
-        let fix go_list_pair ps :=
-            match ps with
-            | [] => []
-            | p :: ps => go_pair p :: go_list_pair ps
-            end in
-        match e with
-        | Value v => Value v
-        | Arg => UpVar 0
-        | UpVar n => UpVar (S n)
-        | Call f a => Call (go f) (go a)
-        | MkConstr tag args => MkConstr tag (go_list args)
-        | ElimBody rec cases => ElimBody (go rec) (go_list_pair cases)
-        | MkClose fname free => MkClose fname (go_list free)
-        end in go.
-
-Definition shift_list :=
-    let go := shift in
-    let fix go_list es :=
-        match es with
-        | [] => []
-        | e :: es => go e :: go_list es
-        end in go_list.
-
-Definition shift_pair :=
-    let go := shift in
-    let fix go_pair (p : expr * rec_info) :=
-        let '(e, r) := p in
-        (go e, r) in go_pair.
-
-Definition shift_list_pair :=
-    let go_pair := shift_pair in
-    let fix go_list_pair ps :=
-        match ps with
-        | [] => []
-        | p :: ps => go_pair p :: go_list_pair ps
-        end in go_list_pair.
-
-Ltac refold_shift :=
-    fold shift_list in *;
-    fold shift_pair in *;
-    fold shift_list_pair in *.
-
-
-
-Definition is_value_dec : forall e : expr, { is_value e } + { ~ is_value e }.
-destruct e; solve [left; constructor | right; inversion 1].
-Defined.
-
-
-
-
-
-Fixpoint upvar_list' acc n :=
-    match n with
-    | 0 => acc
-    | S n' => upvar_list' (UpVar n' :: acc) n'
-    end.
-
-Definition upvar_list n := upvar_list' [] n.
-
-Lemma upvar_list'_length : forall acc n,
-    length (upvar_list' acc n) = length acc + n.
-first_induction n; intros.
-- simpl. lia.
-- simpl. rewrite IHn. simpl. lia.
-Qed.
-
-Lemma upvar_list_length : forall n,
-    length (upvar_list n) = n.
-intros. eapply upvar_list'_length.
-Qed.
-
-Lemma upvar_list'_acc : forall acc n,
-    upvar_list' acc n = upvar_list' [] n ++ acc.
-first_induction n; intros; simpl; eauto.
-- rewrite (IHn [_]). rewrite IHn. rewrite <- app_assoc. simpl. reflexivity.
-Qed.
-
-Lemma upvar_list_tail : forall n,
-    upvar_list (S n) = upvar_list n ++ [UpVar n].
-intros. unfold upvar_list at 1. simpl.
-rewrite upvar_list'_acc. reflexivity.
-Qed.
-
-Lemma upvar_list_nth_error : forall i n,
-    i < n ->
-    nth_error (upvar_list n) i = Some (UpVar i).
-first_induction n; intros0 Hlt.
-  { exfalso. lia. }
-destruct (eq_nat_dec i n).
-- subst i. rewrite upvar_list_tail.
-  rewrite nth_error_app2 by (rewrite upvar_list_length; lia).
-  rewrite upvar_list_length. replace (n - n) with 0 by lia.
-  simpl. reflexivity.
-- assert (i < n) by lia.
-  rewrite upvar_list_tail.
-  rewrite nth_error_app1 by (rewrite upvar_list_length; lia).
-  eauto.
-Qed.
-
-Lemma upvar_list_not_value : forall n,
-    Forall (fun e => ~ is_value e) (upvar_list n).
-intros. eapply nth_error_Forall. intros.
-assert (i < n).
-  { rewrite <- upvar_list_length with (n := n). rewrite <- nth_error_Some.  congruence. }
-rewrite upvar_list_nth_error in * by auto.
-inject_some. inversion 1.
-Qed.
-
-
-
-Definition rec_shape e :=
-    exists fname n, e = MkClose fname (upvar_list n).
-
-Definition elim_rec_shape :=
-    let fix go e :=
-        let fix go_list es :=
-            match es with
-            | [] => True
-            | e :: es => go e /\ go_list es
-            end in
-        let fix go_pair p :=
-            let '(e, r) := p in
-            go e in
-        let fix go_list_pair ps :=
-            match ps with
-            | [] => True
-            | p :: ps => go_pair p /\ go_list_pair ps
-            end in
-        match e with
-        | Value _ => True
-        | Arg => True
-        | UpVar _ => True
-        | Call f a => go f /\ go a
-        | MkConstr _ args => go_list args
-        | ElimBody rec cases => rec_shape rec /\ go rec /\ go_list_pair cases
-        | MkClose _ free => go_list free
-        end in go.
-
-Definition elim_rec_shape_list :=
-    let go := elim_rec_shape in
-    let fix go_list es :=
-        match es with
-        | [] => True
-        | e :: es => go e /\ go_list es
-        end in go_list.
-
-Definition elim_rec_shape_pair :=
-    let go := elim_rec_shape in
-    let fix go_pair (p : expr * rec_info) :=
-        match p with
-        | (e, _) => go e
-        end in go_pair.
-
-Definition elim_rec_shape_list_pair :=
-    let go_pair := elim_rec_shape_pair in
-    let fix go_list_pair ps :=
-        match ps with
-        | [] => True
-        | p :: ps => go_pair p /\ go_list_pair ps
-        end in go_list_pair.
-
-Ltac refold_elim_rec_shape :=
-    fold elim_rec_shape_list in *;
-    fold elim_rec_shape_pair in *;
-    fold elim_rec_shape_list_pair in *.
-
-Lemma elim_rec_shape_list_Forall : forall es,
-    elim_rec_shape_list es <-> Forall elim_rec_shape es.
-induction es; simpl in *; refold_elim_rec_shape; split; intro; eauto.
-- break_and. constructor; firstorder.
-- on >Forall, invc. firstorder.
-Qed.
-
-
-Definition rec_info_eq_dec (x y : rec_info) := list_eq_dec Bool.bool_dec x y.
-
-Definition expr_eq_dec (x y : expr) : { x = y } + { x <> y }.
-make_first x.
-induction x using expr_rect_mut with
-    (Pl := fun x => forall y, { x = y } + { x <> y })
-    (Pp := fun x => forall y, { x = y } + { x <> y })
-    (Plp := fun x => forall y, { x = y } + { x <> y });
-destruct y; try solve [right; inversion 1 | left; auto].
-
-- destruct (value_eq_dec v v0); [ | right; inversion 1; auto ].
-  left. congruence.
-
-- destruct (eq_nat_dec n n0); [ | right; inversion 1; auto ].
-  left. congruence.
-
-- destruct (IHx1 y1); [ | right; inversion 1; auto ].
-  destruct (IHx2 y2); [ | right; inversion 1; auto ].
-  left. congruence.
-
-- destruct (eq_nat_dec tag tag0); [ | right; inversion 1; auto ].
-  destruct (IHx args0); [ | right; inversion 1; auto ].
-  left. congruence.
-
-- destruct (IHx y); [ | right; inversion 1; auto ].
-  destruct (IHx0 cases0); [ | right; inversion 1; auto ].
-  left. congruence.
-
-- destruct (eq_nat_dec f f0); [ | right; inversion 1; auto ].
-  destruct (IHx free0); [ | right; inversion 1; auto ].
-  left. congruence.
-
-- destruct (IHx e); [ | right; inversion 1; auto ].
-  destruct (IHx0 y); [ | right; inversion 1; auto ].
-  left. congruence.
-
-- destruct (IHx e); [ | right; inversion 1; auto ].
-  destruct (rec_info_eq_dec r r0); [ | right; inversion 1; auto ].
-  left. congruence.
-
-- destruct (IHx p0); [ | right; inversion 1; auto ].
-  destruct (IHx0 y); [ | right; inversion 1; auto ].
-  left. congruence.
-
-Defined.
-
-Definition rec_shape_dec (e : expr) : { rec_shape e } + { ~ rec_shape e }.
-destruct e; try solve [right; inversion 1; break_exists; discriminate].
-
-remember (length free) as n.
-destruct (list_eq_dec expr_eq_dec free (upvar_list n)); cycle 1.
-  { right. inversion 1. break_exists.
-    replace x0 with n in *; [ congruence | ].
-    on >@eq, invc. eapply upvar_list_length. }
-left. exists f. exists n. congruence.
-Defined.
-
-Definition elim_rec_shape_dec (e : expr) : { elim_rec_shape e } + { ~ elim_rec_shape e }.
-induction e using expr_rect_mut with
-    (Pl := fun e => { elim_rec_shape_list e } + { ~ elim_rec_shape_list e })
-    (Pp := fun e => { elim_rec_shape_pair e } + { ~ elim_rec_shape_pair e })
-    (Plp := fun e => { elim_rec_shape_list_pair e } + { ~ elim_rec_shape_list_pair e });
-simpl in *; refold_elim_rec_shape; repeat break_and;
-try solve [ assumption | left; eauto ].
-
-- destruct IHe1; [ | right; firstorder ].
-  destruct IHe2; [ | right; firstorder ].
-  left; firstorder.
-
-- destruct (rec_shape_dec e); [ | right; firstorder ].
-  destruct IHe; [ | right; firstorder ].
-  destruct IHe0; [ | right; firstorder ].
-  left; firstorder.
-
-- destruct IHe; [ | right; firstorder ].
-  destruct IHe0; [ | right; firstorder ].
-  left; firstorder.
-
-- destruct IHe; [ | right; firstorder ].
-  destruct IHe0; [ | right; firstorder ].
-  left; firstorder.
-
-Defined.
-
-Definition elim_rec_shape_list_dec (es : list expr) :
-    { elim_rec_shape_list es } + { ~ elim_rec_shape_list es }.
-induction es;
-simpl in *; refold_elim_rec_shape; repeat break_and.
-
-- left. constructor.
-
-- destruct (elim_rec_shape_dec a); [ | right; firstorder ].
-  destruct IHes; [ | right; firstorder ].
-  left; firstorder.
-
-Defined.
-
-
 
