src/ElimFuncComp2.v
@@ -1,1682 +1,388 @@
-Require Import Common Monads.
+Require Import Common.
+
+Require Import Utopia.
 Require Import Metadata.
-Require String.
-Require ElimFunc ElimFunc2.
+Require Import Program.
+Require Import Monads.
+
 Require Import ListLemmas.
-Require Import StepLib.
+Require Import Semantics.
 Require Import HigherValue.
+Require Import StepLib.
 
-Require Import Psatz.
+Require Tagged.
+Require ElimFunc2.
 
-Module A := ElimFunc.
+Module A := Tagged.
 Module B := ElimFunc2.
 
 
-Fixpoint free_list' acc n :=
+
+Definition nth_local n :=
     match n with
-    | 0 => B.Arg :: acc
-    | S n' => free_list' (B.UpVar n' :: acc) n'
+    | 0 => B.Arg
+    | S n => B.UpVar n
     end.
 
-Definition free_list n :=
+Fixpoint locals_list' n acc :=
     match n with
-    | 0 => []
-    | S n => free_list' [] n
+    | 0 => acc
+    | S n => locals_list' n (nth_local n :: acc)
     end.
 
-Definition close_dyn_free drop expect :=
-    skipn drop (free_list (expect + drop)).
+Definition locals_list n := locals_list' n [].
 
 
-Definition compile :=
+Fixpoint free_list' n acc :=
+    match n with
+    | 0 => acc
+    | S n => free_list' n (B.UpVar n :: acc)
+    end.
+
+Definition free_list n := free_list' n [].
+
+
+
+Section compile.
+Open Scope option_monad.
+
+Definition simple_compile : A.expr -> option B.expr :=
     let fix go e :=
         let fix go_list es :=
             match es with
-            | [] => []
-            | e :: es => go e :: go_list es
+            | [] => Some []
+            | e :: es => @cons _ <$> go e <*> go_list es
             end in
-        let fix go_pair p :=
-            let '(e, r) := p in (go e, r) in
-        let fix go_list_pair ps :=
-            match ps with
-            | [] => []
-            | p :: ps => go_pair p :: go_list_pair ps
-            end in
+
         match e with
-        | A.Arg => B.Arg
-        | A.UpVar n => B.UpVar n
-        | A.Call f a => B.Call (go f) (go a)
-        | A.Constr tag args => B.Constr tag (go_list args)
-        | A.ElimBody rec cases => B.ElimBody (go rec) (go_list_pair cases)
-        | A.Close fname free => B.Close fname (go_list free)
-        | A.CloseDyn fname drop expect => B.Close fname (close_dyn_free drop expect)
+        | A.Value v => Some (B.Value v)
+        | A.Arg => Some B.Arg
+        | A.UpVar n => Some (B.UpVar n)
+        | A.Call f a => B.Call <$> go f <*> go a
+        | A.MkConstr tag args => B.MkConstr tag <$> go_list args
+        | A.Elim cases target => None
+        | A.MkClose fname free => B.MkClose fname <$> go_list free
         end in go.
 
-Definition compile_list :=
-    let go := compile in
+Definition simple_compile_list : list A.expr -> option (list B.expr) :=
+    let go := simple_compile in
     let fix go_list es :=
         match es with
-        | [] => []
-        | e :: es => go e :: go_list es
+        | [] => Some []
+        | e :: es => @cons _ <$> go e <*> go_list es
         end in go_list.
 
-Definition compile_pair :=
-    let go := compile in
-    let fix go_pair (p : A.expr * A.rec_info) :=
-        let '(e, r) := p in (go e, r) in go_pair.
+Definition simple_compile_pair : A.expr * A.rec_info -> option (B.expr * B.rec_info) :=
+    let go := simple_compile in
+    let go_pair p :=
+        let '(e, r) := p in
+        go e >>= fun e' => Some (e', r) in go_pair.
 
-Definition compile_list_pair :=
-    let go_pair := compile_pair in
+Definition simple_compile_list_pair :=
+    let go_pair := simple_compile_pair in
     let fix go_list_pair ps :=
         match ps with
-        | [] => []
-        | p :: ps => go_pair p :: go_list_pair ps
+        | [] => Some []
+        | p :: ps => @cons _ <$> go_pair p <*> go_list_pair ps
         end in go_list_pair.
 
-Ltac refold_compile :=
-    fold compile_list in *;
-    fold compile_pair in *;
-    fold compile_list_pair in *.
+Definition compile fname nfrees e : option B.expr :=
+    match e with
+    | A.Elim cases A.Arg =>
+            nth_error nfrees fname >>= fun nfree =>
+            B.Elim (B.MkClose fname (free_list nfree))
+                <$> simple_compile_list_pair cases
+                <*> Some B.Arg
+    | _ => simple_compile e
+    end.
 
 
-Definition compile_func (f : A.expr) : option (B.expr) :=
-    if A.close_dyn_placement_dec f
-        then Some (compile f)
-        else None.
-
-Section compile_cu.
-Open Scope option_monad.
+Definition compile_cu' nfrees es :=
+    map_partial (fun n_e => compile (fst n_e) nfrees (snd n_e)) (numbered es).
 
 Definition compile_cu (cu : list A.expr * list metadata) :
         option (list B.expr * list metadata) :=
-    let '(funcs, metas) := cu in
-    map_partial compile_func funcs >>= fun funcs' =>
-    if B.enough_free_list_dec funcs' funcs'
-        then Some (funcs', metas)
-        else None.
+    let '(exprs, metas) := cu in
+    compile_cu' (map m_nfree metas) exprs >>= fun exprs' =>
+    Some (exprs', metas).
 
-End compile_cu.
+End compile.
 
-
-Lemma compile_list_Forall : forall aes bes,
-    compile_list aes = bes ->
-    Forall2 (fun a b => compile a = b) aes bes.
-induction aes; destruct bes; intros0 Hcomp; simpl in Hcomp; try discriminate.
-- constructor.
-- invc Hcomp. eauto.
-Qed.
-
-Lemma compile_list_length : forall es,
-    length (compile_list es) = length es.
-intros. induction es.
-- reflexivity.
-- simpl. f_equal. eauto.
-Qed.
-
-Lemma compile_list_pair_length : forall es,
-    length (compile_list_pair es) = length es.
-intros. induction es.
-- reflexivity.
-- simpl. f_equal. eauto.
-Qed.
+Ltac refold_simple_compile :=
+    fold simple_compile_list in *;
+    fold simple_compile_pair in *;
+    fold simple_compile_list_pair in *.
 
 
 
-Inductive I_expr (AE : A.env) (BE : B.env) : A.expr -> B.expr -> Prop :=
-| IArg : I_expr AE BE A.Arg B.Arg
-| IUpVar : forall n, I_expr AE BE (A.UpVar n) (B.UpVar n)
+
+(* Steps of elim evaluation:
+
+    Elim cases arg       ~ Elim (MkClose fname (free_list ...)) cases arg
+    Elim cases arg_v     ~ Elim (Value (Close fname locals)) cases arg_v
+        (unroll:)              (unroll:)
+    Elim case arg2       ~ Call (MkClose fname (free_list ...)) arg2
+    Elim case arg2_v     ~ Call (Value (Close fname locals)) arg2_v
+        (unroll:)              (call + unroll:)
+    Elim case arg2       ~ Call (MkClose fname (free_list ...)) arg2
+
+   We handle all of these cases in `I_expr` (instead of in `I`) because after
+   unrolling, they may occur nested under many `Call`s.
+ *)
+
+Definition loop_expr fname (lfree : list value) := B.MkClose fname (free_list (length lfree)).
+Definition loop_value fname lfree := Close fname lfree.
+Definition loop_value_expr fname lfree := B.Value (loop_value fname lfree).
+
+
+Inductive I_expr (BE : B.env) (lfree : list value): A.expr -> B.expr -> Prop :=
+| IValue : forall v, I_expr BE lfree (A.Value v) (B.Value v)
+| IArg : I_expr BE lfree A.Arg B.Arg
+| IUpVar : forall n, I_expr BE lfree (A.UpVar n) (B.UpVar n)
 | ICall : forall af aa bf ba,
-        I_expr AE BE af bf ->
-        I_expr AE BE aa ba ->
-        I_expr AE BE (A.Call af aa) (B.Call bf ba)
-| IConstr : forall tag aargs bargs,
-        Forall2 (I_expr AE BE) aargs bargs ->
-        I_expr AE BE (A.Constr tag aargs) (B.Constr tag bargs)
-| IElimBody : forall arec acases brec bcases,
-        I_expr AE BE arec brec ->
-        Forall2 (fun ap bp => I_expr AE BE (fst ap) (fst bp) /\ snd ap = snd bp) acases bcases ->
-        I_expr AE BE (A.ElimBody arec acases) (B.ElimBody brec bcases)
-| IClose : forall fname afree bfree body,
-        nth_error BE fname = Some body ->
-        let n := length bfree in
-        B.num_locals body <= S n ->
-        n <= length afree ->
-        Forall2 (I_expr AE BE) (firstn n afree) bfree ->
-        (* Additional constraints ensure we avoid matching non-values to values.
-           This only matters after evaluating a CloseDyn, so it's okay. *)
-        Forall A.value (skipn n afree) ->
-        I_expr AE BE (A.Close fname afree) (B.Close fname bfree)
-| ICloseDyn : forall fname adrop aexpect bfree,
-        close_dyn_free adrop aexpect = bfree ->
-        aexpect > 0 ->
-        I_expr AE BE (A.CloseDyn fname adrop aexpect)
-                     (B.Close fname bfree)
-(* Special case for `Call (CloseDyn _ _ 0) _`.  Otherwise we end up matching
- * non-values to values, and all hell breaks loose. *)
-| ICallCdzExpr : forall fname adrop aarg barg,
-        I_expr AE BE aarg barg ->
-        I_expr AE BE (A.Call (A.CloseDyn fname adrop 0) aarg)
-                     (B.Call (B.Close fname []) barg)
-| IElimCdzExpr : forall fname adrop acases bcases,
-        Forall2 (fun ap bp => I_expr AE BE (fst ap) (fst bp) /\ snd ap = snd bp) acases bcases ->
-        I_expr AE BE (A.ElimBody (A.CloseDyn fname adrop 0) acases)
-                     (B.ElimBody (B.Close fname []) bcases)
+        I_expr BE lfree af bf ->
+        I_expr BE lfree aa ba ->
+        I_expr BE lfree (A.Call af aa) (B.Call bf ba)
+| IMkConstr : forall tag aargs bargs,
+        Forall2 (I_expr BE lfree) aargs bargs ->
+        I_expr BE lfree (A.MkConstr tag aargs) (B.MkConstr tag bargs)
+| IMkClose : forall fname aargs bargs,
+        Forall2 (I_expr BE lfree) aargs bargs ->
+        I_expr BE lfree (A.MkClose fname aargs) (B.MkClose fname bargs)
+
+| IElim0 : forall acases atarget bfname bcases btarget,
+        Forall2 (fun ap bp => I_expr BE lfree (fst ap) (fst bp) /\
+                snd ap = snd bp) acases bcases ->
+        I_expr BE lfree atarget btarget ->
+        nth_error BE bfname = Some (B.Elim (loop_expr bfname lfree) bcases B.Arg) ->
+        I_expr BE lfree
+            (A.Elim acases atarget)
+            (B.Elim (loop_expr bfname lfree) bcases btarget)
+
+| IElim1 : forall target acases bfname bcases,
+        Forall2 (fun ap bp => I_expr BE lfree (fst ap) (fst bp) /\
+                snd ap = snd bp) acases bcases ->
+        nth_error BE bfname = Some (B.Elim (loop_expr bfname lfree) bcases B.Arg) ->
+        I_expr BE lfree
+            (A.Elim acases (A.Value target))
+            (B.Elim (loop_value_expr bfname lfree) bcases (B.Value target))
+
+| IElim2 : forall acases atarget bfname bcases btarget,
+        Forall2 (fun ap bp => I_expr BE lfree (fst ap) (fst bp) /\
+                snd ap = snd bp) acases bcases ->
+        I_expr BE lfree atarget btarget ->
+        nth_error BE bfname = Some (B.Elim (loop_expr bfname lfree) bcases B.Arg) ->
+        I_expr BE lfree
+            (A.Elim acases atarget)
+            (B.Call (loop_expr bfname lfree) btarget)
+
+| IElim3 : forall target acases bfname bcases,
+        Forall2 (fun ap bp => I_expr BE lfree (fst ap) (fst bp) /\
+                snd ap = snd bp) acases bcases ->
+        nth_error BE bfname = Some (B.Elim (loop_expr bfname lfree) bcases B.Arg) ->
+        I_expr BE lfree
+            (A.Elim acases (A.Value target))
+            (B.Call (loop_value_expr bfname lfree) (B.Value target))
 .
 
 Inductive I (AE : A.env) (BE : B.env) : A.state -> B.state -> Prop :=
-| IRun : forall ae al ak be bl bk,
-        I_expr AE BE ae be ->
-        Forall A.value al ->
-        Forall B.value bl ->
-        B.num_locals be <= length bl ->
-        length bl <= length al ->
-        Forall2 (I_expr AE BE) (firstn (length bl) al) bl ->
-        (forall av bv,
-            A.value av ->
-            B.value bv ->
-            I_expr AE BE av bv ->
-            I AE BE (ak av) (bk bv)) ->
-        I AE BE (A.Run ae al ak) (B.Run be bl bk)
+| IRun : forall l ae ak be bk,
+        I_expr BE l ae be ->
+        (forall v,
+            I AE BE (ak v) (bk v)) ->
+        I AE BE (A.Run ae l ak) (B.Run be l bk)
 
-(* Special hack for the intermediate state in `Call (CloseDyn _ _ 0) _`
-
-   On the left, 2 steps:                      On the right, no steps:
-         Call (CloseDyn _ _ 0) _        <=>     Call (Close _ [])
-      -> CloseDyn _ _ 0  [k := ...]     <=>     ???
-      -> Call (Close _ []) _            <=>     Call (Close _ [])
-
-   This constructor handles the middle case.
- *)
-| ICallCdz : forall fname drop aarg al ak barg bl bk,
-        I_expr AE BE aarg barg ->
-        Forall A.value al ->
-        Forall B.value bl ->
-        B.num_locals barg <= length bl ->
-        length bl <= length al ->
-        Forall2 (I_expr AE BE) (firstn (length bl) al) bl ->
-        (forall av bv,
-            A.value av ->
-            B.value bv ->
-            I_expr AE BE av bv ->
-            I AE BE (ak av) (bk bv)) ->
-        I AE BE (A.Run (A.CloseDyn fname drop 0) al
-                    (fun av => A.Run (A.Call av aarg) al ak))
-                (B.Run (B.Call (B.Close fname []) barg) bl bk)
-
-| IElimCdz : forall fname drop acases al ak bcases bl bk,
-        Forall2 (fun ap bp => I_expr AE BE (fst ap) (fst bp) /\ snd ap = snd bp) acases bcases ->
-        Forall A.value al ->
-        Forall B.value bl ->
-        S (B.num_locals_list_pair bcases) <= length bl ->
-        length bl <= length al ->
-        Forall2 (I_expr AE BE) (firstn (length bl) al) bl ->
-        (forall av bv,
-            A.value av ->
-            B.value bv ->
-            I_expr AE BE av bv ->
-            I AE BE (ak av) (bk bv)) ->
-        I AE BE (A.Run (A.CloseDyn fname drop 0) al
-                    (fun av => A.Run (A.ElimBody av acases) al ak))
-                (B.Run (B.ElimBody (B.Close fname []) bcases) bl bk)
-
-| IStop : forall ae be,
-        I_expr AE BE ae be ->
-        I AE BE (A.Stop ae) (B.Stop be).
+| IStop : forall v,
+        I AE BE (A.Stop v) (B.Stop v).
 
 
 
-(* `CloseDyn _ _ 0` needs all sorts of special handling, because it `compile`s
- * from non-value to value (`Close _ []` is always a value) *)
-Inductive is_close_dyn_zero : A.expr -> Prop :=
-| IsCloseDynZero : forall fname drop, is_close_dyn_zero (A.CloseDyn fname drop 0).
-
-Definition is_close_dyn_zero_dec (e : A.expr) :
-    { is_close_dyn_zero e } + { ~ is_close_dyn_zero e }.
-destruct e; try solve [right; inversion 1].
-destruct expect; try solve [right; inversion 1].
-left. constructor.
-Qed.
-
-Definition is_close_dyn_zero_state s :=
-    match s with
-    | A.Run e _ _ => is_close_dyn_zero e
-    | A.Stop e => is_close_dyn_zero e
-    end.
+Ltac i_ctor := intros; econstructor; simpl; eauto.
+Ltac i_lem H := intros; eapply H; simpl; eauto.
 
 
-Inductive almost_value : A.expr -> Prop :=
-| AvConstr : forall tag args,
-        Forall almost_value args ->
-        almost_value (A.Constr tag args)
-| AvClose : forall fname free,
-        Forall almost_value free ->
-        almost_value (A.Close fname free)
-| AvCloseDynZero : forall fname drop,
-        almost_value (A.CloseDyn fname drop 0).
-
-Lemma value_almost_value : forall v, A.value v -> almost_value v.
-induction v using A.expr_ind''; inversion 1.
-- constructor. list_magic_on (args, tt).
-- constructor. list_magic_on (free, tt).
-Qed.
-
-
-
-Lemma free_list'_length : forall acc n,
-    length (free_list' acc n) = length acc + S n.
-first_induction n; intros.
-- simpl. lia.
-- simpl. rewrite IHn. simpl. lia.
-Qed.
-
-Lemma free_list_length : forall n, length (free_list n) = n.
-destruct n.
-- reflexivity.
-- eapply free_list'_length.
-Qed.
-
-Lemma close_dyn_free_length : forall drop expect,
-    length (close_dyn_free drop expect) = expect.
-intros. unfold close_dyn_free.
-rewrite skipn_length. rewrite free_list_length. lia.
-Qed.
-
-Lemma close_dyn_free_zero : forall drop, close_dyn_free drop 0 = [].
-intros.
-cut (length (close_dyn_free drop 0) = 0); [ | eapply close_dyn_free_length ].
-intro. destruct (close_dyn_free _ _); simpl in *.
-- reflexivity.
-- discriminate.
-Qed.
-
-Lemma compile_I_expr : forall AE BE ae be,
-    A.close_dyn_placement ae ->
-    B.enough_free BE be ->
-    compile ae = be ->
-    I_expr AE BE ae be.
-intros AE BE.
-induction ae using A.expr_rect_mut with
-    (Pl := fun aes => forall bes,
-        A.close_dyn_placement_list aes ->
-        B.enough_free_list BE bes ->
-        compile_list aes = bes ->
-        Forall2 (I_expr AE BE) aes bes)
-    (Pp := fun ap => forall bp,
-        A.close_dyn_placement_pair ap ->
-        B.enough_free_pair BE bp ->
-        compile_pair ap = bp ->
-        I_expr AE BE (fst ap) (fst bp) /\ snd ap = snd bp)
-    (Plp := fun aps => forall bps,
-        A.close_dyn_placement_list_pair aps ->
-        B.enough_free_list_pair BE bps ->
-        compile_list_pair aps = bps ->
-        Forall2 (fun ap bp => I_expr AE BE (fst ap) (fst bp) /\ snd ap = snd bp) aps bps);
-intros0 Hcdp Hfree Hcomp;
-simpl in Hcomp; refold_compile; try rewrite <- Hcomp; try rewrite <- Hcomp in Hfree;
-simpl in Hfree; B.refold_enough_free BE; repeat (break_exists || break_and);
-invc Hcdp || simpl in Hcdp; try solve [eauto | constructor; eauto].
-
-(* Call case *)
-- destruct ae1; try invc Hcdp; try solve [constructor; eauto; constructor; eauto].
-  destruct expect.
-  + simpl. rewrite close_dyn_free_zero. eapply ICallCdzExpr. eauto.
-  + constructor.
-    * constructor; eauto. lia.
-    * eauto.
-
-(* ElimBody case *)
-- A.refold_close_dyn_placement.
-  destruct ae; break_and; try on (A.close_dyn_placement _), invc;
-    try solve [constructor; eauto; constructor; eauto].
-  destruct expect.
-  + simpl. rewrite close_dyn_free_zero. eapply IElimCdzExpr. eauto.
-  + constructor.
-    * constructor; eauto. lia.
-    * eauto.
-
-(* Close case *)
-- rename x into body. A.refold_close_dyn_placement.
-  rewrite compile_list_length in *.
-  econstructor; eauto.
-  + rewrite compile_list_length. auto.
-  + rewrite compile_list_length. lia.
-  + rewrite compile_list_length. rewrite firstn_all by auto. eapply IHae; eauto.
-  + remember (skipn _ _) as free'.
-    assert (length free' = 0).
-      { subst free'. rewrite skipn_length. rewrite compile_list_length. lia. }
-    destruct free'; try discriminate.
-    constructor.
-
-Qed.
-
-
-Lemma compile_func_close_dyn_placement : forall a b,
-    compile_func a = Some b ->
-    A.close_dyn_placement a.
-intros0 Hcomp.
-unfold compile_func in Hcomp. break_if; try discriminate. inject_some.
-auto.
-Qed.
-
-Theorem compile_cu_close_dyn_placement : forall a ameta b bmeta,
-    compile_cu (a, ameta) = Some (b, bmeta) ->
-    Forall A.close_dyn_placement a.
-intros0 Hcomp. unfold compile_cu in *. break_bind_option.
-  break_if; try discriminate. inject_some.
-on _, apply_lem map_partial_Forall2.
-list_magic_on (a, (b, tt)). eauto using compile_func_close_dyn_placement.
-Qed.
-
-Theorem compile_cu_enough_free : forall a ameta b bmeta,
-    compile_cu (a, ameta) = Some (b, bmeta) ->
-    Forall (B.enough_free b) b.
-intros0 Hcomp. unfold compile_cu in *. break_bind_option.
-  break_if; try discriminate. inject_some.
-rewrite <- B.enough_free_list_Forall. auto.
-Qed.
-
-
-
-
-
-Definition var_n n :=
-    match n with
-    | 0 => B.Arg
-    | S n' => B.UpVar n'
-    end.
-
-Lemma free_list'_nth_error : forall acc n i,
-    (forall j, j < length acc ->
-        nth_error acc j = Some (var_n (S n + j))) ->
-    i < length acc + S n ->
-    nth_error (free_list' acc n) i = Some (var_n i).
-first_induction n; intros0 Hacc Hlt; simpl.
-- destruct i.
-  + simpl. reflexivity.
-  + simpl. rewrite Hacc by lia. simpl. reflexivity.
-- rewrite IHn; [ eauto | | simpl; lia ].
-  intros. simpl in *.
-  destruct j; simpl.
-  + replace (n + 0) with n by lia. reflexivity.
-  + rewrite Hacc by lia. do 2 f_equal. lia.
-Qed.
-
-Lemma free_list_nth_error : forall n i,
-    i < n ->
-    nth_error (free_list n) i = Some (var_n i).
-intros0 Hlt.
-destruct n.
-  { lia. }
-simpl. rewrite free_list'_nth_error; eauto.
-simpl. intros. lia.
-Qed.
-
-Lemma close_dyn_free_nth_error : forall drop expect i,
-    i < expect ->
-    nth_error (close_dyn_free drop expect) i = Some (var_n (drop + i)).
-intros0 Hlt.
-unfold close_dyn_free.
-rewrite skipn_nth_error. rewrite free_list_nth_error by lia.
-reflexivity.
-Qed.
-
-Lemma var_n_num_locals : forall n, B.num_locals (var_n n) = S n.
-destruct n; simpl; reflexivity.
-Qed.
-
-Lemma close_dyn_free_num_locals : forall expect drop,
-    0 < expect ->
-    B.num_locals_list (close_dyn_free drop expect) = drop + expect.
-intros0 Hlt.
-
-rewrite B.num_locals_list_is_maximum.
-fwd eapply close_dyn_free_length with (drop := drop) (expect := expect).
-remember (close_dyn_free _ _) as free.
-
-assert (maximum (map B.num_locals free) <= drop + expect). {
-    rewrite maximum_le_Forall. rewrite <- Forall_map.
-    rewrite Forall_forall. intros0 Hin.
-    eapply In_nth_error in Hin. break_exists.
-    assert (x0 < expect). {
-      erewrite <- close_dyn_free_length with (drop := drop).
-      rewrite <- nth_error_Some. congruence.
-    }
-    subst free. rewrite close_dyn_free_nth_error in * by assumption.
-    inject_some. rewrite var_n_num_locals.
-    lia.
-}
-
-assert (maximum (map B.num_locals free) >= drop + expect). {
-    replace free with (slice 0 expect free); cycle 1.
-      { unfold slice. simpl. rewrite firstn_all by lia. reflexivity. }
-    rewrite slice_split with (k := expect - 1) by lia.
-    rewrite map_app. rewrite maximum_app.
-    replace (expect) with (S (expect - 1)) at 3 by lia.
-    erewrite nth_error_slice; cycle 1.
-      { subst free. eapply close_dyn_free_nth_error. lia. }
-    simpl. rewrite var_n_num_locals.
-    lia.
-}
-
-lia.
-Qed.
-
-Lemma I_expr_value : forall AE BE a b,
-    I_expr AE BE a b ->
-    A.value a ->
-    B.value b.
-induction a using A.expr_ind''; intros0 II Aval; invc II; invc Aval.
-- constructor. list_magic_on (args, (bargs, tt)).
-- constructor.
-  do 2 on (Forall _ free), fun H => eapply Forall_firstn with (n := n) in H.
-  remember (firstn n free) as afree.
-  list_magic_on (afree, (bfree, tt)).
-Qed.
-
-Lemma slice_all : forall A (xs : list A),
-    slice 0 (length xs) xs = xs.
-intros. unfold slice. simpl. rewrite firstn_all by lia. reflexivity.
-Qed.
-
-Lemma I_expr_value' : forall AE BE a b,
-    I_expr AE BE a b ->
-    B.value b ->
-    A.value a.
+Lemma simple_compile_I_expr : forall BE l ae be,
+    simple_compile ae = Some be ->
+    I_expr BE l ae be.
 intros ? ?.
-make_first b.
-induction b using B.expr_ind''; intros0 II Bval; invc II; invc Bval.
-- constructor. list_magic_on (args, (aargs, tt)).
-- constructor. rewrite <- slice_all. rewrite slice_split with (k := length free); cycle 1.
-    { lia. }
-    { erewrite <- Forall2_length by eassumption. rewrite firstn_length. lia. }
-  eapply Forall_app.
-  + rewrite <- firstn_slice. fold n. remember (firstn n afree) as afree'.
-    list_magic_on (afree', (free, tt)).
-  + rewrite <- skipn_slice. assumption.
-- destruct aexpect.
-  + lia.
-  + simpl.
-    fwd eapply Forall_nth_error with (P := B.value) (i := 0) as Hval; eauto.
-      { rewrite close_dyn_free_nth_error by lia. reflexivity. }
-    destruct adrop; simpl in Hval; invc Hval.
-Qed.
+mut_induction ae using A.expr_rect_mut' with
+    (Pl := fun aes => forall bes,
+        simple_compile_list aes = Some bes ->
+        Forall2 (I_expr BE l) aes bes)
+    (Pp := fun ap => forall bp,
+        simple_compile_pair ap = Some bp ->
+        I_expr BE l (fst ap) (fst bp) /\ snd ap = snd bp)
+    (Plp := fun aps => forall bps,
+        simple_compile_list_pair aps = Some bps ->
+        Forall2 (fun ap bp => I_expr BE l (fst ap) (fst bp) /\ snd ap = snd bp) aps bps);
+[ intros0 Hcomp; simpl in *; refold_simple_compile; break_bind_option; inject_some.. | ].
 
-Lemma I_expr_not_value : forall AE BE a b,
-    I_expr AE BE a b ->
-    ~A.value a ->
-    ~B.value b.
-intros. intro. fwd eapply I_expr_value'; eauto.
-Qed.
+- (* Value *) i_ctor.
+- (* Arg *) i_ctor.
+- (* UpVar *) i_ctor.
+- (* Call *) i_ctor.
+- (* MkConstr *) i_ctor.
+- (* Elim *) discriminate.
+- (* MkClose *) i_ctor.
 
-Lemma I_expr_not_value' : forall AE BE a b,
-    I_expr AE BE a b ->
-    ~B.value b ->
-    ~A.value a.
-intros. intro. fwd eapply I_expr_value; eauto.
-Qed.
+- (* nil *) i_ctor.
+- (* cons *) i_ctor.
 
+- (* pair *) i_ctor.
 
+- (* nil *) i_ctor.
+- (* cons *) i_ctor.
 
+- finish_mut_induction simple_compile_I_expr using list pair list_pair.
+Qed exporting.
 
-Ltac B_start HS :=
-    match goal with
-    | [ |- context [ ?pred ?E ?s _ ] ] =>
-            lazymatch pred with
-            | B.sstep => idtac
-            | B.sstar => idtac
-            | B.splus => idtac
-            | _ => fail "unrecognized predicate:" pred
-            end;
-            let S_ := fresh "S" in
-            let S0 := fresh "S" in
-            set (S0 := s);
-            change s with S0;
-            assert (HS : B.sstar E S0 S0) by (eapply B.SStarNil)
-    end.
-
-Ltac B_step HS :=
-    let S_ := fresh "S" in
-    let S2 := fresh "S" in
-    let HS' := fresh HS "'" in
-    let go E s0 s1 Brel solver :=
-        rename HS into HS';
-        evar (S2 : B.state);
-        assert (HS : Brel E s0 S2);
-        [ solver; unfold S2
-        | clear HS' ] in
-    match type of HS with
-    | B.sstar ?E ?s0 ?s1 => go E s0 s1 B.splus
-            ltac:(eapply sstar_then_splus with (1 := HS');
-                  eapply B.SPlusOne)
-    | B.splus ?E ?s0 ?s1 => go E s0 s1 B.splus
-            ltac:(eapply splus_snoc with (1 := HS'))
-    end.
-
-Ltac B_star HS :=
-    let S_ := fresh "S" in
-    let S2 := fresh "S" in
-    let HS' := fresh HS "'" in
-    let go E s0 s1 Brel solver :=
-        rename HS into HS';
-        evar (S2 : B.state);
-        assert (HS : Brel E s0 S2);
-        [ solver; unfold S2
-        | clear HS' ] in
-    match type of HS with
-    | B.sstar ?E ?s0 ?s1 => go E s0 s1 B.sstar
-            ltac:(eapply sstar_then_sstar with (1 := HS'))
-    | B.splus ?E ?s0 ?s1 => go E s0 s1 B.splus
-            ltac:(eapply splus_then_sstar with (1 := HS'))
-    end.
-
-Ltac B_plus HS :=
-    let S_ := fresh "S" in
-    let S2 := fresh "S" in
-    let HS' := fresh HS "'" in
-    let go E s0 s1 Brel solver :=
-        rename HS into HS';
-        evar (S2 : B.state);
-        assert (HS : Brel E s0 S2);
-        [ solver; unfold S2
-        | clear HS' ] in
-    match type of HS with
-    | B.sstar ?E ?s0 ?s1 => go E s0 s1 B.splus
-            ltac:(eapply sstar_then_splus with (1 := HS'))
-    | B.splus ?E ?s0 ?s1 => go E s0 s1 B.splus
-            ltac:(eapply splus_then_splus with (1 := HS'))
-    end.
-
-
-
-
-Lemma nth_error_Some_ex : forall A (xs : list A) n,
-    n < length xs ->
-    exists x, nth_error xs n = Some x.
-intros0 Hlen. rewrite <- nth_error_Some in Hlen.
-destruct (nth_error _ _) eqn:?; try congruence.
-eauto.
+Theorem compile_I_expr : forall BE NFREES l fname ae be,
+    compile fname NFREES ae = Some be ->
+    nth_error BE fname = Some be ->
+    nth_error NFREES fname = Some (length l) ->
+    I_expr BE l ae be.
+destruct ae; intros0 Hcomp Hbe Hnfree; try solve [i_lem simple_compile_I_expr].
+destruct ae; try solve [i_lem simple_compile_I_expr].
+simpl in Hcomp. break_bind_option. inject_some.
+i_ctor. 2: i_ctor.
+i_lem simple_compile_I_expr_list_pair.
 Qed.
 
 
-Definition count_close_dyn_zero :=
-    let fix go e :=
-        let fix go_list es :=
-            match es with
-            | [] => 0
-            | e :: es => go e + go_list es
-            end in
-        let fix go_pair p :=
-            match p with
-            | (e, _) => go e
-            end in
-        let fix go_list_pair ps :=
-            match ps with
-            | [] => 0
-            | p :: ps => go_pair p + go_list_pair ps
-            end in
-        match e with
-        | A.Arg => 0
-        | A.UpVar _ => 0
-        | A.Call f a => go f + go a
-        | A.Constr _ args => go_list args
-        | A.ElimBody rec cases => go rec + go_list_pair cases
-        | A.Close _ free => go_list free
-        | A.CloseDyn _ _ 0 => 1
-        | A.CloseDyn _ _ _ => 0
-        end in go.
 
-Definition count_close_dyn_zero_list :=
-    let go := count_close_dyn_zero in
-    let fix go_list es :=
-        match es with
-        | [] => 0
-        | e :: es => go e + go_list es
-        end in go_list.
 
-Definition count_close_dyn_zero_pair :=
-    let go := count_close_dyn_zero in
-    let fix go_pair (p : A.expr * A.rec_info) :=
-        match p with
-        | (e, _) => go e
-        end in go_pair.
-
-Definition count_close_dyn_zero_list_pair :=
-    let go_pair := count_close_dyn_zero_pair in
-    let fix go_list_pair ps :=
-        match ps with
-        | [] => 0
-        | p :: ps => go_pair p + go_list_pair ps
-        end in go_list_pair.
-
-Ltac refold_count_close_dyn_zero :=
-    fold count_close_dyn_zero_list in *;
-    fold count_close_dyn_zero_pair in *;
-    fold count_close_dyn_zero_list_pair in *.
-
-Definition count_close_dyn_zero_state s :=
-    match s with
-    | A.Run e _ _ => count_close_dyn_zero e
-    | A.Stop e => count_close_dyn_zero e
-    end.
-
-Lemma value_count_close_dyn_zero : forall e,
-    A.value e ->
-    count_close_dyn_zero e = 0.
-induction e using A.expr_rect_mut with
-    (Pl := fun es =>
-        Forall A.value es ->
-        count_close_dyn_zero_list es = 0)
-    (Pp := fun p =>
-        A.value (fst p) ->
-        count_close_dyn_zero_pair p = 0)
-    (Plp := fun ps =>
-        Forall (fun p => A.value (fst p)) ps ->
-        count_close_dyn_zero_list_pair ps = 0);
-inversion 1; simpl; refold_count_close_dyn_zero; eauto.
-all: rewrite (IHe **).
-all: rewrite (IHe0 **).
-all: reflexivity.
+Lemma I_expr_value : forall BE l a b,
+    I_expr BE l a b ->
+    A.is_value a ->
+    B.is_value b.
+intros0 II Aval. invc Aval. invc II. constructor.
 Qed.
+Hint Resolve I_expr_value.
 
-Lemma value_count_close_dyn_zero_list : forall es,
-    Forall A.value es ->
-    count_close_dyn_zero_list es = 0.
-induction es; inversion 1; simpl; refold_count_close_dyn_zero.
+Lemma I_expr_value' : forall BE l a b,
+    I_expr BE l a b ->
+    B.is_value b ->
+    A.is_value a.
+intros0 II Bval. invc Bval. invc II. constructor.
+Qed.
+Hint Resolve I_expr_value'.
+
+Lemma I_expr_not_value : forall BE l a b,
+    I_expr BE l a b ->
+    ~ A.is_value a ->
+    ~ B.is_value b.
+intros0 II Aval. contradict Aval. eauto using I_expr_value'.
+Qed.
+Hint Resolve I_expr_not_value.
+
+Lemma I_expr_not_value' : forall BE l a b,
+    I_expr BE l a b ->
+    ~ B.is_value b ->
+    ~ A.is_value a.
+intros0 II Bval. contradict Bval. eauto using I_expr_value.
+Qed.
+Hint Resolve I_expr_not_value'.
+
+Lemma I_expr_map_value : forall BE l vs bes,
+    Forall2 (I_expr BE l) (map A.Value vs) bes ->
+    bes = map B.Value vs.
+induction vs; intros0 II; invc II.
 - reflexivity.
-- rewrite value_count_close_dyn_zero by assumption.
-  rewrite IHes by assumption.
-  reflexivity.
+- simpl. f_equal.
+  + on >I_expr, invc. reflexivity.
+  + apply IHvs. eauto.
 Qed.
 
 
-Definition A_value_dec : forall e : A.expr, { A.value e } + { ~ A.value e }.
-induction e using A.expr_rect_mut with
-    (Pl := fun es => { Forall A.value es } + { ~ Forall A.value es })
-    (Pp := fun p => { A.value (fst p) } + { ~ A.value (fst p) })
-    (Plp := fun ps => { Forall (fun p => A.value (fst p)) ps } +
-                      { ~ Forall (fun p => A.value (fst p)) ps });
-try solve [left; constructor | right; inversion 1].
-
-- (* constr *)
-  destruct IHe; [ | right; inversion 1; eauto ].
-  left. constructor. eauto.
-
-- (* close *)
-  destruct IHe; [ | right; inversion 1; eauto ].
-  left. constructor. eauto.
-
-- (* cons *)
-  destruct IHe; [ | right; inversion 1; eauto ].
-  destruct IHe0; [ | right; inversion 1; eauto ].
-  left. constructor; eauto.
-
-- (* pair *)
-  simpl. assumption.
-
-- (* cons *)
-  destruct IHe; [ | right; inversion 1; eauto ].
-  destruct IHe0; [ | right; inversion 1; eauto ].
-  left. constructor; eauto.
-Defined.
-
-Definition A_rec_info_eq_dec (x y : A.rec_info) : { x = y } + { x <> y }.
-decide equality. decide equality.
-Defined.
-
-Definition A_expr_eq_dec (x y : A.expr) : { x = y } + { x <> y }.
-generalize dependent y.
-induction x using A.expr_rect_mut with
-    (Pl := fun es => forall es', { es = es' } + { es <> es' })
-    (Pp := fun p => forall p', { p = p' } + { p <> p' })
-    (Plp := fun ps => forall ps', { ps = ps' } + { ps <> ps' });
-intros.
-
-
-- destruct y; try (right; congruence).
-  left. congruence.
-
-- destruct y; try (right; congruence).
-  destruct (eq_nat_dec n n0); try (right; congruence).
-  left. congruence.
-
-- destruct y; try (right; congruence).
-  destruct (IHx1 y1); try (right; congruence).
-  destruct (IHx2 y2); try (right; congruence).
-  left. congruence.
-
-- destruct y; try (right; congruence).
-  destruct (eq_nat_dec tag tag0); try (right; congruence).
-  destruct (IHx args0); try (right; congruence).
-  left. congruence.
-
-- destruct y; try (right; congruence).
-  destruct (IHx y); try (right; congruence).
-  destruct (IHx0 cases0); try (right; congruence).
-  left. congruence.
-
-- destruct y; try (right; congruence).
-  destruct (eq_nat_dec f f0); try (right; congruence).
-  destruct (IHx free0); try (right; congruence).
-  left. congruence.
-
-- destruct y; try (right; congruence).
-  destruct (eq_nat_dec f f0); try (right; congruence).
-  destruct (eq_nat_dec drop drop0); try (right; congruence).
-  destruct (eq_nat_dec expect expect0); try (right; congruence).
-  left. congruence.
-
-
-- destruct es'; try (right; congruence).
-  left. congruence.
-
-- destruct es'; try (right; congruence).
-  destruct (IHx e); try (right; congruence).
-  destruct (IHx0 es'); try (right; congruence).
-  left. congruence.
-
-
-- destruct p'; try (right; congruence).
-  destruct (IHx e); try (right; congruence).
-  destruct (A_rec_info_eq_dec r r0); try (right; congruence).
-  left. congruence.
-
-
-- destruct ps'; try (right; congruence).
-  left. congruence.
-
-- destruct ps'; try (right; congruence).
-  destruct (IHx p0); try (right; congruence).
-  destruct (IHx0 ps'); try (right; congruence).
-  left. congruence.
-Defined.
-
-
-Definition A_matchable s := ~ is_close_dyn_zero_state s.
-
-
-Lemma compile_num_locals : forall a b,
-    compile a = b ->
-    A.num_locals a = B.num_locals b.
-induction a using A.expr_rect_mut with
-    (Pl := fun a => forall b,
-        compile_list a = b ->
-        A.num_locals_list a = B.num_locals_list b)
-    (Pp := fun a => forall b,
-        compile_pair a = b ->
-        A.num_locals_pair a = B.num_locals_pair b)
-    (Plp := fun a => forall b,
-        compile_list_pair a = b ->
-        A.num_locals_list_pair a = B.num_locals_list_pair b);
-intros0 Hcomp;
-simpl in *; refold_compile; A.refold_num_locals;
-subst; simpl; B.refold_num_locals.
-
-- reflexivity.
-- reflexivity.
-- erewrite IHa1, IHa2; reflexivity.
-- erewrite IHa; reflexivity.
-- erewrite IHa, IHa0; reflexivity.
-- erewrite IHa; reflexivity.
-- break_if.
-  + subst. rewrite close_dyn_free_zero. reflexivity.
-  + rewrite close_dyn_free_num_locals by lia. reflexivity.
-
-- reflexivity.
-- erewrite IHa, IHa0; reflexivity.
-
-- eauto.
-
-- reflexivity.
-- erewrite IHa, IHa0; reflexivity.
-Qed.
-
-
-Lemma unroll_elim_sim : forall AE BE,
-    forall arec brec acase bcase aargs bargs ainfo binfo ae',
-    A.unroll_elim arec acase aargs ainfo = Some ae' ->
-    I_expr AE BE arec brec ->
-    I_expr AE BE acase bcase ->
-    Forall2 (I_expr AE BE) aargs bargs ->
-    ainfo = binfo ->
-    exists be',
-        B.unroll_elim brec bcase bargs binfo = Some be' /\
-        I_expr AE BE ae' be'.
-first_induction aargs; destruct ainfo; intros0 Aunroll IIrec IIcase IIargs IIinfo;
-  try discriminate.
-
-- invc IIargs.
-  eexists. split. reflexivity.
-  simpl in Aunroll. inject_some. assumption.
-
-- invc IIargs. simpl. eapply IHaargs; try eassumption; eauto.
-  destruct b; eauto using ICall.
-Qed.
-
-
-Ltac max_split :=
-    repeat match goal with | [ |- _ /\ _ ] => split end.
-
-
-Fixpoint metric e :=
-    match e with
-    | A.ElimBody (A.CloseDyn _ _ _) _ => 2
-    | A.Call (A.CloseDyn _ _ _) _ => 2
-    | A.CloseDyn _ _ _ => 1
-    | _ => 0
-    end.
-
-Definition state_metric s :=
-    match s with
-    | A.Run e _ _ => metric e
-    | A.Stop e => metric e
-    end.
-
-Lemma compile_list_nth_error : forall aes ae n be,
-    nth_error aes n = Some ae ->
-    nth_error (compile_list aes) n = Some be ->
-    compile ae = be.
-intros. remember (compile_list aes) as bes eqn:Hcomp.
-symmetry in Hcomp. eapply compile_list_Forall in Hcomp.
-eapply Forall2_nth_error with (1 := Hcomp); eassumption.
-Qed.
-
-Lemma nth_error_le_maximum_map : forall A f xs (x : A) n,
-    nth_error xs n = Some x ->
-    f x <= maximum (map f xs).
-induction xs; intros0 Hnth.
-- destruct n; discriminate.
-- destruct n; simpl in *.
-  + inject_some. lia.
-  + specialize (IHxs ?? ?? **). lia.
-Qed.
-
-Lemma B_num_locals_case_le_maximum : forall bcases n p,
-    nth_error bcases n = Some p ->
-    B.num_locals_pair p <= B.num_locals_list_pair bcases.
-first_induction bcases; intros0 Hnth; simpl in *.
-- destruct n; discriminate.
-- destruct n; simpl in *.
-  + inject_some. lia.
-  + specialize (IHbcases ?? ?? **). lia.
-Qed.
-
-
-
-Lemma B_close_eval_sliding : forall E i fname free vs es l k,
-    i < length free ->
-    length vs = length es ->
-    Forall B.value vs ->
-    Forall (fun e => ~ B.value e) es ->
-    sliding i vs es free ->
-    (forall i e v,
-        nth_error es i = Some e ->
-        nth_error vs i = Some v ->
-        forall k', B.sstep E (B.Run e l k') (k' v)) ->
-    exists free',
-        B.sstar E (B.Run (B.Close fname free)  l k)
-                  (B.Run (B.Close fname free') l k) /\
-        sliding (S i) vs es free'.
-intros0 Hlen Hlen' Hval Hnval Hsld Hstep.
-
-destruct (nth_error free i) as [e |] eqn:He; cycle 1.
-  { exfalso. rewrite <- nth_error_Some in Hlen. congruence. }
-
-assert (nth_error es i = Some e). {
-  erewrite <- sliding_nth_error_ge; try eassumption. lia.
-}
-
-fwd eapply length_nth_error_Some.
-  { symmetry. eassumption. }
-  { eassumption. }
-destruct ** as [v Hv].
-
-erewrite sliding_split with (xs1 := vs) (xs2 := es) (ys := free); try eassumption.
-B_start HS.
-
-B_step HS.
-  { eapply B.SCloseStep.
-    - eapply Forall_firstn. eassumption.
-    - eapply Forall_nth_error with (1 := Hnval). eassumption.
-  }
-
-B_step HS.
-  { eapply Hstep; eauto. }
-
-eapply splus_sstar in HS.
-eexists. split. eapply HS.
-eapply sliding_app; eauto.
-eapply sliding_length in Hsld; eauto. congruence.
-Qed.
-
-
-Lemma B_close_eval_sliding' : forall E fname l k  j i free vs es,
-    i + j = length free ->
-    i < length free ->
-    length vs = length es ->
-    Forall B.value vs ->
-    Forall (fun e => ~ B.value e) es ->
-    sliding i vs es free ->
-    (forall i e v,
-        nth_error es i = Some e ->
-        nth_error vs i = Some v ->
-        forall k', B.sstep E (B.Run e l k') (k' v)) ->
-    B.sstar E (B.Run (B.Close fname free)  l k)
-              (B.Run (B.Close fname vs) l k).
-induction j; intros0 Hi Hlt Hlen Hval Hnval Hsld Hstep.
-{ lia. }
-
-(* Give explicit instantiations, otherwise lia breaks with "abstract cannot
-   handle existentials" *)
-fwd eapply B_close_eval_sliding with (E := E) (fname := fname) (k := k); eauto.
-  destruct ** as (free' & Hstep' & Hsld').
-
-assert (length free = length vs) by eauto using sliding_length.
-assert (length free' = length vs) by eauto using sliding_length.
-
-destruct (eq_nat_dec (S i) (length free)) as [Hlen' | Hlen'].
-{ (* easy case: that was the last free variable, nothing more to eval *)
-  destruct Hsld' as [Hpre' Hsuf'].
-  replace (S i) with (length free') in Hpre' at 1 by congruence.
-  replace (S i) with (length vs) in Hpre' at 1 by congruence.
-  do 2 rewrite firstn_all in Hpre' by reflexivity.
-  rewrite <- Hpre'. assumption.
-}
-
-specialize (IHj (S i) free' vs es ltac:(lia) ltac:(lia) ** ** ** ** **).
-
-eapply sstar_then_sstar; eassumption.
-Qed.
-
-
-
-Lemma B_close_eval_cdf : forall E fname drop expect l k,
-    0 < expect ->
-    drop + expect <= length l ->
-    Forall B.value l ->
-    B.sstar E (B.Run (B.Close fname (close_dyn_free drop expect)) l k)
-              (B.Run (B.Close fname (firstn expect (skipn drop l))) l k).
-intros0 Hnonzero Hllen Hlval.
-eapply B_close_eval_sliding' with (i := 0) (j := expect) (es := close_dyn_free drop expect).
-- rewrite close_dyn_free_length. lia.
-- rewrite close_dyn_free_length. lia.
-- rewrite firstn_length. rewrite skipn_length. rewrite close_dyn_free_length. lia.
-- eauto using Forall_firstn, Forall_skipn.
-- eapply nth_error_Forall. intros0 Hnth.
-  rewrite close_dyn_free_nth_error in Hnth; cycle 1.
-    { rewrite <- close_dyn_free_length with (drop := drop) (expect := expect).
-      rewrite <- nth_error_Some. congruence. }
-  inject_some. destruct (drop + i); inversion 1.
-- eapply sliding_zero.
-- intros0 He Hv. intros.
-  assert (i < expect).
-    { rewrite <- close_dyn_free_length with (drop := drop) (expect := expect).
-      rewrite <- nth_error_Some. congruence. }
-  rewrite close_dyn_free_nth_error in He by auto. inject_some.
-  rewrite firstn_nth_error_lt in Hv by auto.
-  rewrite skipn_nth_error in Hv.
-  destruct (drop + i); eauto using B.SArg, B.SUpVar.
-Qed.
-
-Lemma firstn_app' : forall A (xs ys : list A) n,
-    n >= length xs ->
-    firstn n (xs ++ ys) = xs ++ firstn (n - length xs) ys.
-induction xs; intros0 Hge; simpl in *.
-- replace (n - 0) with n by lia. reflexivity.
-- destruct n; simpl in *. { lia. }
-  rewrite IHxs by lia. reflexivity.
-Qed.
 
 Theorem I_sim : forall AE BE a a' b,
-    compile_list AE = BE ->
-    Forall A.close_dyn_placement AE ->
-    Forall (B.enough_free BE) BE ->
+    Forall2 (fun ae be => forall l,
+        (* TODO: premise *)
+        I_expr BE l ae be) AE BE ->
     I AE BE a b ->
     A.sstep AE a a' ->
-    B.enough_free_state BE b ->
     exists b',
-        (B.splus BE b b' \/
-         (b' = b /\ state_metric a' < state_metric a)) /\
+        B.sstep BE b b' /\
         I AE BE a' b'.
-
-destruct a as [ae al ak | ae];
-intros0 Henv Acdp Bef_env II Astep Bef; [ | solve [invc Astep] ].
-
-destruct ae; inv Astep; invc II; [ try on (I_expr _ _ _ _), invc.. | | ].
-
+destruct a as [ae al ak | v];
+intros0 Henv II Astep; inv Astep.
+all: invc II.
+all: try on (I_expr _ _ _ be), invc.
 
 - (* SArg *)
-  fwd eapply nth_error_Some_ex with (n := 0) (xs := bl) as HH.
-    { simpl in *. lia. }
-    destruct HH as [bv ?].
-
-  B_start HS.
-  B_step HS. { eapply B.SArg. eassumption. }
-
-  eexists. split; eauto. 
-  eapply H10. (* TODO - need a structtact for this *)
-  + eapply Forall_nth_error; eauto.
-  + eapply Forall_nth_error; eauto.
-  + eapply Forall2_nth_error; eauto.
-    rewrite firstn_nth_error_lt by (rewrite <- nth_error_Some; congruence).
-    assumption.
+  eexists. split. i_lem B.SArg.
+  auto.
 
 - (* SUpVar *)
-  fwd eapply nth_error_Some_ex with (n := S n) (xs := bl) as HH.
-    { simpl in *. lia. }
-    destruct HH as [bv ?].
-
-  B_start HS.
-  B_step HS. { eapply B.SUpVar. eassumption. }
-
-  eexists. split; eauto.
-  eapply H10. (* TODO - need a structtact for this *)
-  + eapply Forall_nth_error; eauto.
-  + eapply Forall_nth_error; eauto.
-  + eapply Forall2_nth_error; eauto.
-    rewrite firstn_nth_error_lt by (rewrite <- nth_error_Some; congruence).
-    assumption.
-
-- (* SCallL *)
-  B_start HS.
-  B_step HS. { eapply B.SCallL. eauto using I_expr_not_value. }
-
-  eexists. split. left. exact HS.
-  unfold S1. constructor; eauto.
-    { simpl in *. lia. }
-  intros. constructor; eauto.
-    { constructor; eauto. }
-    { simpl in *. rewrite B.value_num_locals by assumption. lia. }
-
-- (* SCallL - CDZ *)
-  eexists. split. right. split.
-    { reflexivity. }
-    { simpl. lia. }
-  eapply ICallCdz; eauto.
-
-- (* SCallR *)
-  B_start HS.
-  B_step HS. { eapply B.SCallR; eauto using I_expr_value, I_expr_not_value. }
-
-  eexists. split. left. exact HS.
-  unfold S1. constructor; eauto.
-    { simpl in *. lia. }
-  intros. constructor; eauto.
-    { constructor; eauto. }
-    { simpl in *. rewrite B.value_num_locals with (e := bv) by assumption. lia. }
-
-- (* SCallR - CDZ *)
-  on (A.value (A.CloseDyn _ _ _)), invc.
-
-- (* SMakeCall *)
-  on (I_expr _ _ (A.Close _ _) _), invc.  rename body0 into bbody.
-  remember (firstn n free) as free'.
-  assert (Forall A.value free') by (subst free'; eauto using Forall_firstn).
-
-  B_start HS.
-  B_step HS.
-    { eapply B.SMakeCall; eauto using I_expr_value.
-      list_magic_on (free', (bfree, tt)). eauto using I_expr_value. }
-
-  eexists. split. left. exact HS.
-  unfold S1. constructor; simpl; eauto.
-  * eapply Forall2_nth_error with (x := body) (y := bbody); cycle 1; eauto.
-    remember (compile_list AE) as BE.
-    symmetry in HeqBE. eapply compile_list_Forall in HeqBE.
-    list_magic_on (AE, (BE, tt)).
-    eapply compile_I_expr; eapply Forall_nth_error + idtac; solve [eauto].
-  * constructor; try list_magic_on (bfree, (free', tt)); eauto using I_expr_value.
-  * fold n. lia.
-  * constructor; eauto. subst free'. assumption.
-
-- (* SConstrStep *)
-  on (Forall2 _ (_ ++ _ :: _) _), invc_using Forall2_3part_inv.
-
-  B_start HS.
-  B_step HS.
-    { eapply B.SConstrStep; eauto using I_expr_not_value.
-      list_magic_on (vs, (ys1, tt)). eauto using I_expr_value. }
-
-  simpl in *. B.refold_num_locals. rewrite B.num_locals_list_is_maximum in *.
-  rewrite map_app, map_cons in *. rewrite maximum_app in *. simpl in *.
-
-  eexists. split. left. exact HS.
-  unfold S1. constructor; simpl; eauto.
-    { lia. }
-  intros. constructor; eauto.
-    { constructor; eauto using Forall2_app. }
-    { simpl. B.refold_num_locals. rewrite B.num_locals_list_is_maximum.
-      rewrite map_app, map_cons. rewrite maximum_app. simpl.
-      erewrite B.value_num_locals by eassumption. lia. }
-
-- (* SConstrDone *)
-  B_start HS.
-  B_step HS.
-    { eapply B.SConstrDone. list_magic_on (args, (bargs, tt)). eauto using I_expr_value. }
-
-  eexists. split. left. exact HS.
-  unfold S1. eapply H10; constructor; eauto.
-  + list_magic_on (args, (bargs, tt)). eauto using I_expr_value.
-
-- (* SElimStepRec *)
-  B_start HS.
-  B_step HS.
-    { eapply B.SElimStepRec. eauto using I_expr_not_value. }
-
-  eexists. split. left. exact HS.
-  unfold S1. constructor; eauto.
-    { simpl in *. B.refold_num_locals. lia. }
-  intros. constructor; eauto.
-    { constructor; eauto. }
-    { simpl in *. rewrite B.value_num_locals by assumption. lia. }
-
-- (* SElimStepRec - CDZ *)
-  eexists. split. right. split.
-    { reflexivity. }
-    { simpl. lia. }
-  eapply IElimCdz; eauto.
-    { simpl in *. B.refold_num_locals. lia. }
-
-- (* SEliminate *)
-  destruct bl as [ | bv bl].
-    { simpl in *. B.refold_num_locals. lia. }
-  on (Forall2 _ _ (bv :: bl)), invc.
-  on (I_expr _ _ _ bv), invc.
-
-  fwd eapply length_nth_error_Some as HH; [ | eassumption | ].
-    { eapply Forall2_length. eassumption. }
-    destruct HH as [[bcase binfo] ?].
-
-  replace binfo with info in *; cycle 1.
-    { on (Forall2 _ _ bcases), fun H => fwd eapply Forall2_nth_error with (1 := H); eauto.
-      simpl in *.  firstorder. }
-
-  fwd eapply unroll_elim_sim as HH; eauto.
-    { on (Forall2 _ _ bcases), fun H => fwd eapply Forall2_nth_error with (1 := H); eauto.
-      simpl in *. firstorder eauto. }
-    destruct HH as [be' [? ?]].
-
-
-  B_start HS.
-  B_step HS.
-    { eapply B.SEliminate; eauto using I_expr_value.
-      list_magic_on (args, (bargs, tt)). eauto using I_expr_value. }
-
-  on (Forall A.value _), invc.
-  on (Forall B.value _), invc.
-
-  eexists. split. left. exact HS.
-  unfold S1. constructor; eauto.
-  + simpl in *. B.refold_num_locals.
-    fwd eapply B.unroll_elim_num_locals; eauto. simpl in *.
-    assert (B.num_locals brec = 0).
-      { eapply B.value_num_locals. eauto using I_expr_value. }
-    assert (B.num_locals_pair (bcase, info) <= B.num_locals_list_pair bcases).
-      { eauto using B_num_locals_case_le_maximum. }
-    assert (B.num_locals_list bargs <= 0).
-      { rewrite B.num_locals_list_is_maximum. rewrite maximum_le_Forall.
-        rewrite <- Forall_map.
-        on (B.value (B.Constr _ _)), invc.
-        list_magic_on (bargs, tt).
-        rewrite B.value_num_locals by auto. lia. }
-    simpl in *. lia.
-  + simpl in *. lia.
-
-- (* SEliminate - CDZ *)
-  on (A.value (A.CloseDyn _ _ _)), invc.
+  eexists. split. i_lem B.SUpVar.
+  auto.
 
 - (* SCloseStep *)
-  (* The element of `free` to be evaluated (`e`) must left of `n`, so `firstn` will keep it. *)
-  assert (n >= S (length vs)). {
-    destruct (ge_dec n (S (length vs))). { eassumption. }
-    exfalso. assert (n <= length vs) by lia.
-    rewrite skipn_app_l in * by auto.
-    on (Forall A.value (_ ++ _)), invc_using Forall_app_inv.
-    on (Forall A.value (e :: _)), invc.
-    eauto.
-  }
-
-  change (e :: es) with ([e] ++ es) in *.
-  rewrite firstn_app', firstn_app' in * by (simpl; lia).
-  remember (firstn _ es) as es'.
-  assert (n = length (vs ++ [e] ++ es')).
-    { fwd eapply Forall2_length; eauto. }
-  assert (length es' <= length es).
-    { repeat rewrite app_length in *. simpl in *. lia. }
-
-  simpl in *. B.refold_num_locals.
-  on (Forall2 _ (_ ++ _ :: _) _), fun H => inversion H using Forall2_3part_inv.
-  intros. subst bfree.
-
-  B_start HS.
-  B_step HS.
-    { eapply B.SCloseStep; eauto using I_expr_not_value.
-      list_magic_on (vs, (ys1, tt)). eauto using I_expr_value. }
-
-  rewrite B.num_locals_list_is_maximum in *.
-  rewrite map_app, map_cons in *. rewrite maximum_app in *. simpl in *.
-
-  eexists. split. left. exact HS.
-  unfold S1. constructor; simpl; eauto.
-    { lia. }
-  intros. constructor; eauto.
-    { collect_length_hyps.
-      econstructor; eauto.
-      - rewrite app_length in *. simpl in *. congruence.
-      - repeat rewrite app_length in *. simpl in *. omega.
-      - rewrite firstn_app' by (rewrite app_length; simpl; omega).
-        change (av :: es) with ([av] ++ es).
-        rewrite firstn_app' by (rewrite app_length; simpl; omega).
-        replace (firstn _ es) with es'; cycle 1.
-          { subst es'. unfold n. f_equal. do 2 rewrite app_length. simpl. reflexivity. }
-        eapply Forall2_app; eauto. constructor; eauto.
-      - replace (length _) with n; cycle 1.
-          { unfold n. do 2 rewrite app_length. simpl. omega. }
-        rewrite skipn_app in * by omega.
-        change (av :: es) with ([av] ++ es).
-        change (e :: es) with ([e] ++ es) in *.
-        rewrite skipn_app in * by (simpl; omega).
-        simpl in *. assumption.
-    }
-    { simpl. B.refold_num_locals. rewrite B.num_locals_list_is_maximum.
-      rewrite map_app, map_cons. rewrite maximum_app. simpl.
-      erewrite B.value_num_locals by eassumption. lia. }
+  on _, invc_using Forall2_3part_inv.
+  eexists. split. i_lem B.SCloseStep.
+  + list_magic_on (vs, (ys1, tt)).
+  + i_ctor. i_ctor. i_ctor. i_lem Forall2_app. i_ctor. i_ctor.
 
 - (* SCloseDone *)
-  remember (firstn n free) as free'.
-  assert (Forall A.value free') by (subst free'; eauto using Forall_firstn).
-
-  B_start HS.
-  B_step HS.
-    { eapply B.SCloseDone. list_magic_on (free', (bfree, tt)). eauto using I_expr_value. }
-
-  eexists. split. left. exact HS.
-  unfold S1. eapply H10; econstructor; eauto.
-  + list_magic_on (free', (bfree, tt)). eauto using I_expr_value.
-  + fold n. congruence.
-
-- (* SCloseDyn *)
-  simpl in *. B.refold_num_locals.
-  rewrite close_dyn_free_num_locals in * by lia.
-
-  invc Bef. on (B.enough_free _ _), invc. B.refold_enough_free (compile_list AE).
-  break_exists. break_and. rename x into bbody. rewrite close_dyn_free_length in *.
-
-  B_start HS.
-  B_star HS.
-    { eapply B_close_eval_cdf; eauto. }
-  B_step HS.
-    { eapply B.SCloseDone. eauto using Forall_firstn, Forall_skipn. }
-
-
-  eexists. split. left. exact HS.
-  unfold S2. eapply H9; eauto.
-  + constructor. eauto using Forall_skipn.
-  + constructor. eauto using Forall_firstn, Forall_skipn.
-  + econstructor; eauto using Forall_firstn, Forall_skipn.
-    * rewrite firstn_length, skipn_length. lia.
-    * rewrite firstn_length, skipn_length, skipn_length. lia.
-    * rewrite firstn_length, skipn_length.
-      replace (min _ _) with expect by lia.
-      erewrite <- firstn_firstn with (m := length bl - drop) by lia.
-      rewrite firstn_skipn_swap. replace (length bl - drop + drop) with (length bl) by lia.
-      eauto using Forall2_firstn, Forall2_skipn.
-
-- (* SCloseDyn - Call CDZ *)
-  invc Bef. simpl in *. B.refold_enough_free (compile_list AE).
-  repeat (break_and || break_exists). rename x into bbody.
-
-  eexists. split. right. split.
-    { reflexivity. }
-    { simpl. lia. }
-  constructor; eauto.
-  constructor; eauto.
-  econstructor; simpl; eauto using Forall_skipn.  lia.
-
-- (* SCloseDyn - Elim CDZ *)
-  invc Bef. simpl in *. B.refold_enough_free (compile_list AE).
-  repeat (break_and || break_exists). rename x into bbody.
-
-  eexists. split. right. split.
-    { reflexivity. }
-    { simpl. lia. }
-  constructor; eauto.
-  constructor; eauto.
-  econstructor; simpl; eauto using Forall_skipn.
-    { lia. }
-    { simpl. B.refold_num_locals. lia. }
-
-Qed.
-
-
-Inductive I' (AE : A.env) (BE : B.env) : A.state -> B.state -> Prop :=
-| I'_intro : forall a b,
-        I AE BE a b ->
-        B.enough_free_state BE b ->
-        I' AE BE a b.
-
-Theorem I'_sim : forall AE BE a a' b,
-    compile_list AE = BE ->
-    Forall A.close_dyn_placement AE ->
-    Forall (B.enough_free BE) BE ->
-    I' AE BE a b ->
-    A.sstep AE a a' ->
-    exists b',
-        (B.splus BE b b' \/
-         (b' = b /\ state_metric a' < state_metric a)) /\
-        I' AE BE a' b'.
-intros. on >I', invc.
-fwd eapply I_sim; eauto. break_exists; break_and.
-eexists; split; eauto. constructor; eauto.
-eapply B.enough_free_star; try eassumption.
-- on (_ \/ _), invc.
-  + eapply splus_sstar. auto.
-  + break_and. subst. eapply SStarNil.
-Qed.
-
-
-
-
-
-Require Semantics.
-
-Ltac i_ctor := intros; econstructor; eauto.
-Ltac i_lem H := intros; eapply H; eauto.
-
-Lemma compile_cu_compile_list : forall a ameta b bmeta,
-    compile_cu (a, ameta) = Some (b, bmeta) ->
-    compile_list a = b.
-intros.
-simpl in *. break_bind_option. break_if; try discriminate. inject_some.
-on _, apply_lem map_partial_Forall2.
-on >B.enough_free_list, fun H => clear H.
-generalize dependent b. induction a; intros; on >Forall2, invc.
-- simpl. reflexivity.
-- simpl. f_equal; eauto.
-  unfold compile_func in *. break_if; try discriminate. inject_some. reflexivity.
-Qed.
-
-Lemma compile_cu_Forall : forall A Ameta B Bmeta,
-    compile_cu (A, Ameta) = Some (B, Bmeta) ->
-    Forall2 (fun a b => compile a = b) A B.
-intros.
-eapply compile_list_Forall.
-eapply compile_cu_compile_list. eauto.
-Qed.
-
-Lemma compile_cu_metas : forall A Ameta B Bmeta,
-    compile_cu (A, Ameta) = Some (B, Bmeta) ->
-    Ameta = Bmeta.
-simpl. inversion 1. break_bind_option.
-do 2 (break_match; try discriminate). inject_some. auto.
-Qed.
-
-(* `match_values` is the relevant parts of `I_expr` lifted to `HigherValue.value`s *)
-Inductive match_values (AE : A.env) (BE : B.env) (M : list metadata) : value -> value -> Prop :=
-| MvConstr : forall tag aargs bargs,
-        Forall2 (match_values AE BE M) aargs bargs ->
-        match_values AE BE M (Constr tag aargs) (Constr tag bargs)
-| MvClose : forall fname afree bfree body,
-        nth_error BE fname = Some body ->
-        let n := length bfree in
-        B.num_locals body <= S n ->
-        n <= length afree ->
-        Forall2 (match_values AE BE M) (firstn n afree) bfree ->
-        (* This hack is used for the callstate case.  We need to show that the
-           A-side value is public_value, but there might be values in `afree`
-           that aren't in `bfree`, for which we have no guarantees. *)
-        (Forall (public_value M) bfree -> Forall (public_value M) afree) ->
-        match_values AE BE M (Close fname afree) (Close fname bfree)
-.
-
-
-Lemma match_values_public : forall A B M bv av,
-    match_values A B M av bv ->
-    public_value M bv ->
-    public_value M av.
-intros until M.
-mut_induction bv using value_rect_mut' with
-    (Pl := fun bv => forall av,
-        Forall2 (match_values A B M) av bv ->
-        Forall (public_value M) bv ->
-        Forall (public_value M) av);
-[ intros0 Hmv Bpub; invc Hmv; invc Bpub; i_ctor.. | ].
-- finish_mut_induction match_values_public using list.
-Qed exporting.
-
-Lemma match_values_enough_free : forall A B M,
-    Forall2 (fun a b => compile a = b) A B ->
-    forall av bv be,
-    match_values A B M av bv ->
-    B.expr_value be bv ->
-    B.enough_free B be.
-intros0 Hcomp.
-mut_induction av using value_rect_mut' with
-    (Pl := fun avs => forall n bvs bes,
-        Forall2 (match_values A B M) (firstn n avs) bvs ->
-        Forall2 B.expr_value bes bvs ->
-        Forall (B.enough_free B) bes);
-[ intros0 Hmval Bev.. | ];
-[ invc Hmval; invc Bev.. | | | ].
-
-- simpl. B.refold_enough_free B. rewrite B.enough_free_list_Forall.
-  fwd eapply IHav; eauto.
-  erewrite firstn_all by eauto. auto.
-
-- simpl. B.refold_enough_free B. rewrite B.enough_free_list_Forall.
-  fwd eapply IHav; eauto.
-  split; eauto.
-  eexists. split; eauto.
-  collect_length_hyps. subst n. omega.
-
-- destruct n; invc Hmval; invc Bev; auto.
-
-- destruct n; invc Hmval; invc Bev; eauto.
-
-- finish_mut_induction match_values_enough_free using list.
-Qed exporting.
-
-
-Lemma A_expr_value_ex : forall av,
-    exists ae, A.expr_value ae av.
-mut_induction av using value_rect_mut' with
-    (Pl := fun avs => exists aes, Forall2 A.expr_value aes avs).
-
-- destruct IHav.
-  eexists. i_ctor.
-
-- destruct IHav.
-  eexists. i_ctor.
-
-- eauto.
-
-- destruct IHav, IHav0.
-  eauto.
-
-- finish_mut_induction A_expr_value_ex using list.
-Qed exporting.
-
-Lemma match_values_I_expr : forall A B M,
-    Forall2 (fun a b => compile a = b) A B ->
-    forall av be bv,
-    B.expr_value be bv ->
-    match_values A B M av bv ->
-    exists ae,
-        A.expr_value ae av /\
-        I_expr A B ae be.
-make_first bv. intros0 Hcomp. move bv at bottom.
-mut_induction bv using value_rect_mut' with
-    (Pl := fun bvs => forall n avs bes,
-        Forall2 B.expr_value bes bvs ->
-        Forall2 (match_values A B M) (firstn n avs) bvs ->
-        exists aes,
-            Forall2 A.expr_value aes avs /\
-            Forall2 (I_expr A B) (firstn n aes) bes);
-[intros0 Bev Hmval.. | ].
-
-- invc Bev. invc Hmval.
-  fwd eapply IHbv as HH ; eauto.
-    { erewrite firstn_all by eauto. eauto. }
-    destruct HH as (? & ? & Hfa).
-  eexists. split; i_ctor.
-  + rewrite firstn_all in Hfa by (collect_length_hyps; congruence).
-    auto.
-
-- invc Bev. invc Hmval.
-  fwd eapply IHbv as HH; eauto.
-    destruct HH as (? & ? & Hfa).
-  eexists. split; i_ctor.
-  + collect_length_hyps. rewrite firstn_length, min_l in * by auto. omega.
-  + collect_length_hyps. rewrite firstn_length, min_l in * by auto. omega.
-  + subst n. collect_length_hyps. congruence.
-  + eapply Forall_skipn. eapply A.expr_value_value_list. eauto.
-
-- destruct (A_expr_value_ex_list avs) as (aes & ?).
-  eexists; split; eauto.
-  assert (HH : firstn n aes = []).
-    { destruct aes. { destruct n; reflexivity. }
-      on (Forall2 _ (_ :: _) _), invc.
-      destruct n; simpl in *. { reflexivity. }
-      invc Hmval. }
-  rewrite HH. invc Bev. constructor.
-
-- destruct n; try solve [invc Hmval].
-  destruct avs as [| av avs]; try solve [invc Hmval]. simpl in Hmval.
-  invc Bev. invc Hmval.
-
-  destruct (IHbv ?? ?? ** **) as (? & ? & ?).
-  destruct (IHbv0 ?? ?? ?? ** **) as (? & ? & ?).
-  eexists (_ :: _). simpl. eauto.
-
-- finish_mut_induction match_values_I_expr using list.
-Qed exporting.
-
-Lemma I_expr_match_values : forall A B M,
-    Forall2 (fun a b => compile a = b) A B ->
-    forall av ae be,
-    A.expr_value ae av ->
-    public_value M av ->
-    I_expr A B ae be ->
-    exists bv,
-        B.expr_value be bv /\
-        match_values A B M av bv /\
-        public_value M bv.
-intros0 Hcomp.
-induction av using value_rect_mut with
-    (Pl := fun avs => forall n aes bes,
-        Forall2 A.expr_value aes avs ->
-        Forall (public_value M) avs ->
-        Forall2 (I_expr A B) (firstn n aes) bes ->
-        exists bvs,
-            Forall2 B.expr_value bes bvs /\
-            Forall2 (match_values A B M) (firstn n avs) bvs /\
-            Forall (public_value M) bvs);
-intros0 Aev Apub II.
-
-all: unfold A.valtype, B.valtype in *.
-
-- invc Aev. invc II. invc Apub.
-  fwd eapply IHav as HH ; eauto.
-    { erewrite firstn_all by eauto. eauto. }
-    destruct HH as (? & ? & Hfa & ?).
-  eexists. split; [|split]; i_ctor.
-  + rewrite firstn_all in Hfa by (collect_length_hyps; congruence).
-    auto.
-
-- invc Aev. invc II. invc Apub.
-  fwd eapply IHav as HH; eauto.
-    destruct HH as (? & ? & Hfa & ?).
-  eexists. split; [|split]; i_ctor.
-  + collect_length_hyps. rewrite firstn_length, min_l in * by auto. omega.
-  + collect_length_hyps. rewrite firstn_length, min_l in * by auto. omega.
-  + subst n. collect_length_hyps. congruence.
-
-- invc Aev. destruct n; invc II; simpl; eauto.
-
-- invc Aev. destruct n; invc II; invc Apub; simpl; eauto.
-  destruct (IHav ?? ?? ** ** **) as (? & ? & ? & ?).
-  destruct (IHav0 ?? ?? ?? ** ** **) as (? & ? & ? & ?).
-  eexists. split; [|split]; i_ctor.
-Qed.
-
-
-
-Section Preservation.
-
-  Variable prog : A.prog_type.
-  Variable tprog : B.prog_type.
-
-  Hypothesis TRANSF : compile_cu prog = Some tprog.
-
-  Theorem fsim :
-    Semantics.forward_simulation (A.semantics prog) (B.semantics tprog).
-  Proof.
-    destruct prog as [A Ameta], tprog as [B Bmeta].
-    fwd eapply compile_cu_close_dyn_placement; eauto.
-    fwd eapply compile_cu_enough_free; eauto.
-    fwd eapply compile_cu_Forall; eauto.
-    fwd eapply compile_cu_metas; eauto.
-
-    eapply Semantics.forward_simulation_star with
-        (match_states := I' A B)
-        (match_values := match_values A B Ameta).
-
-    - simpl. intros. on >B.is_callstate, invc. simpl in *.
-      fwd eapply Forall2_nth_error_ex' with (xs := A) (ys := B) as HH; eauto.
-        destruct HH as (abody & ? & ?).
-
-      fwd eapply match_values_I_expr with (bv := av2) as HH; eauto.
-        destruct HH as (av1_e & ? & ?).
-      on (match_values _ _ _ _ (Close _ _)), invc.
-      fwd eapply match_values_I_expr_list with (avs := afree) as HH; eauto.
-        destruct HH as (afree_e & ? & ?).
-
-      eexists. split. 1: econstructor.
-      + econstructor.
-        * i_lem compile_I_expr; i_lem Forall_nth_error.
-        * instantiate (1 := av1_e :: afree_e).
-          eauto using A.expr_value_value_list.
-        * eauto using B.expr_value_value, B.expr_value_value_list.
-        * simpl. subst n. collect_length_hyps. congruence.
-        * simpl. collect_length_hyps.
-          rewrite firstn_length, min_l in * by auto. omega.
-        * simpl. i_ctor.
-          collect_length_hyps. subst n. congruence.
-        * i_ctor.
-
-
-      + i_ctor.
-        * i_lem Forall_nth_error.
-        * constructor.
-          -- eapply match_values_enough_free; [ | | eassumption ]; eauto.
-          -- eapply match_values_enough_free_list; eauto.
-        * i_ctor.
-
-      + i_ctor.
-        * on (public_value _ (Close _ _)), invc. i_ctor.
-        * i_lem match_values_public.
-
-    - intros0 II Afinal. invc Afinal. invc II. on >I, invc.
-      fwd eapply I_expr_match_values as HH; eauto.
-        destruct HH as (bv & ? & ? & ?).
-      eexists. split; eauto.
-      i_ctor.
-
-    - intros0 Astep. intros0 II.
-      eapply sstar_semantics_sim, I'_sim; try eassumption.
-      + eapply compile_cu_compile_list; eauto.
-    Defined.
-
-    Lemma match_val_eq :
-      Semantics.fsim_match_val _ _ fsim = match_values (fst prog) (fst tprog) (snd prog).
-    Proof.
-      unfold fsim. simpl.
-      unfold Semantics.fsim_match_val.
-      break_match. repeat (break_match_hyp; try congruence).
-      try unfold forward_simulation_step in *.
-      try unfold forward_simulation_plus in *.
-      try unfold forward_simulation_star in *.
-      try unfold forward_simulation_star_wf in *.
-      inv Heqf. reflexivity.
-  Qed.
-
-End Preservation.
+  fwd i_lem I_expr_map_value. subst.
+  eexists. split. i_lem B.SCloseDone.
+  auto.
+
+- (* SConstrStep *)
+  on _, invc_using Forall2_3part_inv.
+  eexists. split. i_lem B.SConstrStep.
+  + list_magic_on (vs, (ys1, tt)).
+  + i_ctor. i_ctor. i_ctor. i_lem Forall2_app. i_ctor. i_ctor.
+
+- (* SCloseDone *)
+  fwd i_lem I_expr_map_value. subst.
+  eexists. split. i_lem B.SConstrDone.
+  auto.
+
+- (* SCallL *)
+  eexists. split. i_lem B.SCallL.
+  i_ctor. i_ctor. i_ctor. i_ctor.
+
+- (* SCallR *)
+  eexists. split. i_lem B.SCallR.
+  i_ctor. i_ctor. i_ctor. i_ctor.
+
+- (* SMakeCall *)
+  on (I_expr _ _ _ bf), invc.
+  on (I_expr _ _ _ ba), invc.
+  fwd eapply Forall2_nth_error_ex with (ys := BE) as HH; eauto.
+    destruct HH as (bbody & ? & ?).
+
+  eexists. split. i_lem B.SMakeCall.
+  i_ctor.
+
+- (* SElimStep (IElim0) *)
+  admit.
+
+- (* SElimStep (IElim1) *)
+  on (~ A.is_value (A.Value _)), contradict. i_ctor.
+
+- (* SElimStep (IElim2) *)
+  admit.
+
+- (* SElimStep (IElim3) *)
+  on (~ A.is_value (A.Value _)), contradict. i_ctor.
+
+- (* SEliminate (IElim0) *)
+  admit.
+
+- (* SEliminate (IElim1) *)
+  admit.
+
+- (* SEliminate (IElim2) *)
+  admit.
+
+- (* SEliminate (IElim3) *)
+  admit.
+
+Admitted.
+
+  
+    
+
+
